src/coq/optimisations/maps.v
@@ -8,7 +8,7 @@ Require Import Vellvm.optimisations.EqNat.
 Require Import Vellvm.DecidableEquality.
 Require Import Coq.Logic.FunctionalExtensionality.
 Require Import Coqlib.
-
+Require Import Vellvm.optimisations.map_spec.
 Require Import paco.
 Require Import Vellvm.Memory.
 Require Import Vellvm.Effects.
@@ -19,14 +19,16 @@ Local Unset Case Analysis Schemes.
 Set Implicit Arguments.
 
 
-Require Import compcert.lib.Maps.
 
-Definition test (a b:pc):= decide (a = b).
 
+
+
+Print test.
 
 Module PCTree <: TREE.
   Definition elt := pc.
-  Definition elt_eq := test.
+  Definition pc_eq (a b: pc):= decide (a = b).
+  Definition elt_eq := pc_eq.
   Definition tree A := list (elt * option A).
   Definition t := tree.
 
@@ -61,7 +63,10 @@ Module PCTree <: TREE.
 
 
   Theorem gss : forall (A : Type) (i : pc) (x : A) (m: t A), get i (set i x m) = Some x.
-  Proof. Admitted.
+  Proof. induction m; simpl in *; eauto. destruct (elt_eq i i); eauto. contradiction n; eauto. destruct a; simpl in *. destruct ( elt_eq e i); subst; eauto. simpl in *.
+         destruct ( elt_eq i i ); eauto. contradiction n; eauto. simpl in *. destruct (elt_eq e i); subst. contradiction n; eauto. eauto. 
+  Qed.
+
 
   Lemma gleaf : forall (A : Type) (i : pc), get i (nil : t A) = None.
   Proof. intros. simpl in *. eauto. Qed. Hint Resolve gleaf.
@@ -127,7 +132,7 @@ Hint Resolve grs.
 
     Definition beq_single (a b :(elt * option A)) : bool :=
       match a, b with
-      | (key, None), (key1, None) => elt_eq key key1
+      | (key, None), (key1, None) => (elt_eq key key1)
       | (key, Some a), (key1, Some a1) => (elt_eq key key1) && (beqA a a1)
       | _, _ => false
       end.
@@ -143,10 +148,6 @@ Hint Resolve grs.
       end.
     
     
-    Lemma bempty_correct:
-      forall m, bempty m = true <-> (forall x, get x m = None).
-    Proof. Admitted.
-
 
     Lemma beq_correct: forall m1 m2, beq m1 m2 = true <-> (forall (x: elt),
                                                               match get x m1, get x m2 with
@@ -200,56 +201,63 @@ Print t.
     Variable f: option A -> option B -> option C.
     Hypothesis f_none_none: f None None = None.
 
+Print t.
 
-    Fixpoint xcombine_l (m1 : t A) : t C :=
-      match m1 with
-      | nil => nil
-      | (key, item) :: tl => (key, f item None) :: xcombine_l tl
-      end.
+Print tree.
 
-    Lemma xgcombine_l :
-      forall (m: t A) (i : pc),
-        get i (xcombine_l m) = f (get i m) None.
-    Proof.
-      induction m; intros; simpl in *. eauto. simpl in *. destruct a. simpl in *. destruct ( elt_eq e i). eauto. simpl in *. eauto. Qed.
-
-    Fixpoint xcombine_r (m : t B) : t C :=
-      match m with
-      | nil => nil
-      | (key, item) :: tl => (key, f None item) :: xcombine_r tl
-      end.
-
-    Lemma xgcombine_r :
-      forall (m: t B) (i: pc),
-        get i (xcombine_r m) = f None (get i m).
-    Proof. intros. induction m; simpl in *; eauto.
-           destruct a. simpl in *. destruct (elt_eq e i). eauto. eauto. Qed.
-
-
-    Fixpoint combine (m1: t A) (m2: t B) : t C :=
-      match m1, m2 with
-      | nil, nil => nil
-      | nil, list => xcombine_r list
-      | list, nil => xcombine_l list
-      | (key, item)::tl, (key1, item1)::tl1 => (key, (f item item1)) :: combine tl tl1
+  Fixpoint xcombine_l (m : t A) {struct m} : t C :=
+    match m with
+    | nil => nil
+               | (key, val) :: tl => (key, (f val None)) :: xcombine_l tl
+    (*  | Leaf => Leaf
+      | Node l o r => Node' (xcombine_l l) (f o None) (xcombine_l r)*)
       end.
 
 
-    Theorem gcombine:
-      forall (m1: t A) (m2: t B) (i: pc),
-        get i (combine m1 m2) = f (get i m1) (get i m2).
-      Proof. induction m1. simpl in *. induction m2. simpl in *. auto. simpl in *. 
-             intros. destruct a. simpl in *. destruct ( elt_eq e i); simpl in *; eauto. induction m2. simpl in *; eauto. simpl in *. destruct a. simpl in *. specialize (IHm2 i). auto.
-             simpl in *. destruct a. simpl in *. induction m2. simpl in *. intros. destruct (elt_eq e i). eauto. induction m1. simpl in *. auto. simpl in *. destruct a. simpl in *.
+  Lemma xgcombine_l :
+          forall m i,
+          get i (xcombine_l m) = f (get i m) None.
+Proof.
+      induction m; intros; simpl; symmetry; eauto. destruct a. simpl in *. remember ( elt_eq e i). destruct s. simpl in *. eauto. symmetry. eauto. Qed.
+
+  Fixpoint xcombine_r (m : t B) {struct m} : t C :=
+    match m with
+    | nil => nil
+    | (key, val) :: tl => (key, (f None val)) :: xcombine_r tl
+      end.
+
+
+  Lemma xgcombine_r :
+          forall m i,
+          get i (xcombine_r m) = f None (get i m).
+Proof.
+      induction m; intros; simpl; symmetry; eauto. destruct a. simpl in *. remember ( elt_eq e i). destruct s. simpl in *. eauto. symmetry. eauto. Qed.
 
 
 
+Fixpoint combine (l1: t A) (l2: t B) :=
+  match l1 with
+  | nil => xcombine_r l2
+  | (a, b) :: tl => match get a l2 with
+                       | None => (a, f b None) :: combine tl (remove a l2)
+                       | Some res => (a, f b (Some res)) :: combine tl (remove a l2)
+                       end
+                         
+                       
+  end.
 
 
-             destruct (elt_eq e0 i). eauto. apply IHm0. simpl in *. Admitted.
+
+Theorem gcombine:
+      forall m1 m2 i,
+      get i (combine m1 m2) = f (get i m1) (get i m2).
+Proof. 
+ Admitted.
+
+
 
 End COMBINE.
-      
+     
 
   Fixpoint elements A (m : t A) : (list (pc * A)) :=
     match m with
@@ -268,7 +276,12 @@ End COMBINE.
   Theorem elements_complete:
     forall (A: Type) (m: t A) (i: pc) (v: A),
       In (i, v) (elements m) -> get i m = Some v.
-  Proof. induction m. intros. simpl in *. inversion H. intros. simpl in *.  Admitted.
+  Proof. induction m. intros. simpl in *. inversion H. intros. simpl in *.   destruct a.
+destruct ( elt_eq e i).
+
+
+
+  Admitted.
 
 
 
@@ -327,13 +340,14 @@ Theorem fold1_spec:
   forall (A B: Type) (f: B -> A -> B) (v: B) (m: t A),
     fold1 f m v =
     List.fold_left (fun a p => f a (snd p)) (elements m) v.
-  Proof. Admitted.
+  Proof. Admitted. 
 End PCTree.
 
-
+  
 Module PCMap <: MAP.
   Definition elt := pc.
-  Definition elt_eq := test.
+  Definition pc_eq (a b:pc) := decide (a = b).
+  Definition elt_eq := pc_eq.
 
   Definition t (A : Type) : Type := (A * PCTree.t A)%type.
 
@@ -368,9 +382,9 @@ Module PCMap <: MAP.
 
   Theorem gsspec:
     forall (A: Type) (i j: pc) (x: A) (m: t A),
-      get i (set j x m) = if elt_eq i j then x else get i m.
-  Proof. intros.  destruct (elt_eq i j). subst. apply gss. rewrite gso. auto. auto. Qed.
-
+      get i (set j x m) = if pc_eq i j then x else get i m.
+  Proof. intros.  destruct (elt_eq i j). subst. simpl in *. unfold get, set. simpl in *. destruct ( pc_eq j j). simpl in *. rewrite PCTree.gss. eauto. contradiction n; eauto.
+ unfold get, set. simpl in *. destruct ( pc_eq i j). subst. contradiction n. auto. eapply PCTree.gso in n. rewrite n. eauto. Qed.
 
 
   Theorem gsident:
@@ -395,827 +409,438 @@ Module PCMap <: MAP.
   Theorem set2:
     forall (A: Type) (i: elt) (x y: A) (m: t A),
       set i y (set i x m) = set i y m.
-  Proof.
-    intros. unfold set. simpl in *. decEq. Admitted.
+  Proof. induction m; simpl in *. unfold set. simpl in *. induction b. simpl in *. destruct (PCTree.elt_eq i i). eauto. contradiction n; eauto.
+         simpl in *. destruct a0. simpl in *. destruct ( PCTree.elt_eq e i). subst. simpl in *. destruct ( PCTree.elt_eq i i ). eauto. contradiction n. eauto.
+         simpl in *. destruct (PCTree.elt_eq e i). subst. contradiction n; eauto. inversion IHb. rewrite H0. eauto. Qed.
 End PCMap.
   
+
 
 
 Notation "a ! b" := (PCTree.get b a) (at level 1).
 Notation "a !! b" := (PCMap.get b a) (at level 1).
 
-(*
-  
-  Definition elt := pc.
-  Definition pc_comp (A B:pc) : bool := decide (A = B).
-  Print pc_comp.
-  Definition elt_eq := pc_comp.
 
 
 
-  Definition t A := seq (pc * option A).
+
+(*********)
+
+
+
+Definition loc_id_eq (a b:local_id) := decide (a = b).
+
+Module lidTree <: TREE.
+  Definition elt := local_id.
+  Definition elt_eq := loc_id_eq.
+  Definition tree A := list (elt * option A).
+  Definition t := tree.
+
 
   Definition empty (A : Type) := (nil : t A).
-  Print elt_eq.
+Print elt_eq.
   
-  Fixpoint get (A : Type) (p : pc) (m : t A) : option A :=
+  Fixpoint get (A:Type) (i:local_id) (m: t A) : option A :=
     match m with
     | nil => None
-    | hd :: tl => if (elt_eq (fst hd) p) then (snd hd) else get  p tl
+    | (key, item) :: tl => if (elt_eq key i) then item else get i tl
     end.
 
-
-  Fixpoint get (A : Type) (i : pc) (v : A) (m : t A) : t A :=
+  Fixpoint set (A: Type) (i: local_id) (v:A) (m : t A) : t A :=
     match m with
     | nil => cons (i, Some v) nil
-    | hd :: tl  => if (elt_eq (fst hd) i) then (i, Some v) :: tl else hd :: (set i v tl)
+    | (key, item) :: tl => if (elt_eq key i) then (key, Some v) :: tl  else (key, item) :: set i v tl
     end.
 
-
-  Fixpoint remove (A : Type) (p : pc) (m : t A) : t A :=
+  Fixpoint remove (A : Type) (i : local_id) (m : t A) : t A :=
     match m with
     | nil => nil
-    | hd :: tl => if (elt_eq (fst hd) p) then remove p tl else hd :: (remove p tl)
+    | (key, item) :: tl => if (elt_eq key i) then remove i tl else (key, item) :: remove i tl
     end.
 
 
+  Theorem gempty :
+    forall (A : Type) (i : local_id), get i (empty A) = None.
+  Proof. intros. simpl in *. eauto. Qed.
+  Hint Resolve gempty.
 
-  Lemma eq_refl : forall i, elt_eq i i = true.
-  Proof. intros. unfold elt_eq. unfold pc_comp. destruct ( decide (i = i)). simpl in *. eauto. contradiction n. eauto. Qed.
-Hint Rewrite eq_refl.
-  
-      Theorem gempty:
-    forall (A: Type) (i: pc), get i (empty A) = None.
-Proof. move => //. Qed.
 
-  Theorem gss:
-    forall (A: Type) (i: pc) (x: A) (m:t A), get i (set i x m) = Some x.
-  Proof. intros. induction m; simpl in *. rewrite eq_refl. eauto. simpl in *. destruct a. simpl in *. unfold elt_eq. unfold pc_comp. unfold is_left. simpl in *. destruct ( decide (p = i)); simpl in *; eauto. rewrite eq_refl. eauto. simpl in *. unfold elt_eq. simpl in *. unfold pc_comp. simpl in *. unfold is_left. destruct (decide (p = i)); subst. contradiction n; eauto. eauto. Qed.
 
-Hint Resolve gss.
+  Theorem gss : forall (A : Type) (i : local_id) (x : A) (m: t A), get i (set i x m) = Some x.
+  Proof.
+    intros. induction m; simpl in *. destruct ( elt_eq i i). eauto. contradiction n; eauto. destruct a. simpl in *.
+    destruct ( elt_eq e i). subst. simpl in *. destruct (elt_eq i i). eauto. contradiction n; eauto. simpl in *.
+    destruct ( elt_eq e i). subst. contradiction n ; eauto. eauto.
+  Qed.
 
-         
-    Lemma gleaf : forall (A : Type) (i : pc), get i (nil : t A) = None.
-    Proof. intros. simpl in *. auto. Qed.
-Hint Resolve gleaf.
-    
-  Theorem gso:
-    forall (A: Type) (i j: pc) (x: A) (m: t A),
-    i <> j -> get i (set j x m) = get i m.
-  Proof. intros. induction m. simpl in *.
-         +unfold elt_eq. simpl in *. unfold pc_comp. unfold is_left. destruct ( decide (j = i)). subst. contradiction H; eauto. eauto.
-         +simpl in *. unfold elt_eq. simpl in *. unfold pc_comp. simpl in *. unfold is_left. simpl in *. destruct a. simpl in *.
-          destruct ( decide (p = j)). simpl in *; subst. unfold elt_eq. unfold pc_comp. unfold is_left. simpl in *. destruct ( decide (j = i)); subst. contradiction H. eauto. eauto.
-         +simpl in *. unfold elt_eq. simpl in *. unfold pc_comp. simpl in *. unfold is_left. simpl in *. destruct ( decide (p = i)); subst. eauto. simpl in *. eauto. Qed.
+
+  Lemma gleaf : forall (A : Type) (i : local_id), get i (nil : t A) = None.
+  Proof. intros. simpl in *. eauto. Qed. Hint Resolve gleaf.
+
+
+  Theorem gso : forall (A : Type) (i j : local_id) (x: A) (m : t A), i <> j -> get i (set j x m) = get i m.
+  Proof. intros. induction m; simpl in *. destruct ( elt_eq j i). subst. contradiction H; eauto. eauto.
+
+         destruct a. simpl in *. destruct ( elt_eq e j). simpl in *. subst. destruct ( elt_eq j i); subst. contradiction H; eauto. eauto. simpl in *. destruct (elt_eq e i). eauto. eauto. Qed.
 Hint Resolve gso.
-         
-  Theorem gsspec:
-    forall (A: Type) (i j: pc) (x: A) (m: t A),
-    get i (set j x m) = if elt_eq i j then Some x else get i m.
-Proof.
-  intros. unfold elt_eq. unfold pc_comp. unfold is_left. simpl in *. destruct ( decide (i = j)). subst. auto. auto. Qed.
-Hint Resolve gsspec.
-
-
   
-  Theorem gsident:
-    forall (A: Type) (i: pc) (m: t A) (v: A),
-      get i m = Some v -> set i v m = m.
-  Proof. intros. induction m; simpl in *; eauto.
+  Theorem gsspec : forall (A : Type) (i j: local_id) (x : A) (m: t A), get i (set j x m) = if (elt_eq i j) then Some x else get i m.
+  Proof. intros. induction m; simpl in *; eauto. destruct (elt_eq j i). destruct (elt_eq i j); subst; eauto. contradiction n; eauto. destruct (elt_eq i j); subst; eauto. contradiction n; eauto.
+
+
+         destruct a. destruct (elt_eq e j). simpl in *. subst. destruct ( elt_eq j i). subst. destruct (elt_eq i i); eauto. contradiction n; eauto. simpl in *. eauto. simpl in *. destruct ( elt_eq i j); subst. contradiction n; eauto. eauto. simpl in *. destruct ( elt_eq e i); subst. destruct (elt_eq i j). subst. contradiction n; eauto. eauto. eauto. Qed. Hint Resolve gsspec.
+
+
+  Theorem gsident: forall (A: Type) (i: local_id) (m: t A) (v: A), get i m = Some v -> set i v m = m.
+  Proof. intros. induction m; simpl in *.
          +inversion H.
-         +destruct a. unfold elt_eq in *. unfold pc_comp in *. simpl in *. unfold is_left in *. simpl in *. destruct ( decide (p = i)); subst; eauto. simpl in *. apply IHm in H. rewrite H; eauto. Qed.
-Hint Resolve gsident.
+         +simpl in *. destruct a. simpl in *. destruct (elt_eq e i). subst. simpl in *. eauto. apply IHm in H. rewrite H. auto. Qed. Hint Resolve gsident.
 
-
-
-  Theorem set2:
-    forall (A: Type) (i: elt) (m: t A) (v1 v2: A),
-    set i v2 (set i v1 m) = set i v2 m.
-  Proof. intros. induction m. simpl in *. rewrite  eq_refl; eauto. simpl in *. destruct a. simpl in *. unfold elt_eq. simpl in *. unfold pc_comp. simpl in *. unfold is_left. simpl in *. destruct ( decide (p = i)). simpl in *. rewrite eq_refl.
-eauto. simpl in *. unfold elt_eq. simpl in *. unfold pc_comp. unfold is_left.  destruct ( decide (p = i)); subst. contradiction n; eauto. rewrite IHm. eauto. Qed. Hint Rewrite set2.
-
-    
-  Lemma rleaf : forall (A : Type) (i : pc), remove i (nil : t A) = nil.
-Proof. intros. simpl in *. eauto. Qed. Hint Rewrite rleaf.  Hint Resolve rleaf.
 
   Theorem grs:
-    forall (A: Type) (i: pc) (m: t A), get i (remove i m) = None.
-Proof.
-  intros. simpl in *. induction m.
-  +simpl in *. eauto.
-  +simpl in *. destruct a. simpl in *. unfold elt_eq. unfold pc_comp. unfold is_left. destruct (decide (p = i)). eauto.  simpl in *. unfold elt_eq. unfold pc_comp. unfold is_left. destruct (decide (p = i)); subst. contradiction n. eauto. eauto. Qed.
-  Hint Resolve grs.
+    forall (A: Type) (i: local_id) (m: t A), get i (remove i m) = None.
+  Proof. intros. induction m. simpl in *. auto. simpl in *.
+         destruct a. simpl in *. destruct ( elt_eq e i).
+         subst. auto. simpl in *. destruct (elt_eq e i).
+         subst. contradiction n. auto. auto. Qed.
+Hint Resolve grs.
+
+
   Theorem gro:
-    forall (A: Type) (i j: pc) (m: t A),
-    i <> j -> get i (remove j m) = get i m.
-  Proof. 
-    intros.  induction m; simpl in *; eauto. destruct a. unfold elt_eq. unfold pc_comp. unfold is_left. simpl in *. destruct (decide (p = j)); subst. destruct ( decide (j = i)); subst. contradiction H; eauto. eauto. simpl in *. unfold elt_eq. unfold pc_comp. unfold is_left. destruct ( decide (p = i) ); eauto. Qed.
-  Hint Resolve gro.
-  
-  
-  Theorem grspec:
-    forall (A: Type) i j (m: t A),
-    get i (remove j m) = if elt_eq i j then None else get i m.
-  Proof. induction m. simpl in *. unfold elt_eq. simpl in *. unfold pc_comp. unfold is_left. simpl in *. 
-destruct ( decide (i = j)); eauto. unfold elt_eq in *. unfold pc_comp in *. unfold is_left in *. simpl in *. destruct a. simpl in *. unfold elt_eq. unfold pc_comp in *. unfold is_left in *. destruct (decide (p = j)); simpl in *; subst; eauto.
-destruct ( decide (i = j)); subst; eauto. destruct ( decide (j = i) ); subst; eauto. contradiction n; eauto. unfold elt_eq. unfold pc_comp in *. unfold is_left in *. destruct ( decide (p = i)); subst; eauto. destruct ( decide (i = j)); simpl in *; subst; eauto. contradiction n. eauto. Qed. Hint Resolve grspec.
+    forall (A: Type) (i j: local_id) (m: t A),
+      i <> j -> get i (remove j m) = get i m.
+  Proof. intros. induction m. simpl in *. auto. simpl in *. destruct a. simpl in *.
+         destruct ( elt_eq e j). subst. destruct ( elt_eq j i). subst.
+         contradiction H; eauto.  eauto. simpl in *.
+         destruct (elt_eq e i). auto. eauto.
+  Qed. Hint Resolve gro.
 
 
-
+  Theorem grspec: forall (A: Type) (i j: elt) (m: t A), get i (remove j m) = if elt_eq i j then None else get i m.
+  Proof. intros. induction m. simpl in *. destruct (elt_eq i j). eauto.
+         eauto. simpl in *. destruct a. simpl in *.
+         destruct ( elt_eq e j), (elt_eq i j); subst; eauto.
+         destruct ( elt_eq j i); subst. contradiction n; eauto.
+         eauto. simpl in *. destruct ( elt_eq e j); subst; eauto. contradiction n; eauto.
+         simpl in *. destruct ( elt_eq e i); eauto.
+         Qed.
 
   Section BOOLEAN_EQUALITY.
 
     Variable A: Type.
     Variable beqA: A -> A -> bool.
-    Print t.
 
-    Definition single_empty (a : (pc * option A)) :=
+
+    Definition bsingle_empty A (a: (elt * option A)) :=
       match a with
-      | (_, Some _) => false
-      | _ => true
+      | (key, Some item) => true
+      | _ => false
+               
       end.
-
     
     Fixpoint bempty (m: t A) : bool :=
       match m with
       | nil => true
-      | hd :: tl => single_empty hd && bempty tl
+      | hd :: tl => bsingle_empty hd && bempty tl
       end.
 
-      Definition single_eq (a b : (pc * option A)) :=
+
+    Definition beq_single (a b :(elt * option A)) : bool :=
       match a, b with
-      | (pc1, Some op1), (pc2, Some op2) => elt_eq pc1 pc2 && beqA op1 op2
-      | (pc1, None), (pc2, None) => elt_eq pc1 pc2
+      | (key, None), (key1, None) => elt_eq key key1
+      | (key, Some a), (key1, Some a1) => (elt_eq key key1) && (beqA a a1)
       | _, _ => false
       end.
+    
+                
 
-        
-    Fixpoint beq (m1 m2: t A) {struct m1} : bool :=
+    Fixpoint beq (m1 m2: t A) : bool :=
       match m1, m2 with
       | nil, nil => true
-      | hd1::tl1, hd2::tl2  => single_eq hd1 hd2 && beq tl1 tl2
-      | _, _ => false
-                  
+      | _, nil => bempty m1
+      | nil, _ => bempty m2
+      | hd::tl, hd1::tl1 =>  beq_single hd hd1 && beq tl tl1                 
       end.
-
+    
+    
     Lemma bempty_correct:
       forall m, bempty m = true <-> (forall x, get x m = None).
-    Proof. intros; split; intros.
-           +induction m. simpl in *. auto. simpl in *. destruct a. simpl in *. unfold elt_eq.  
-            unfold pc_comp in *. unfold is_left. destruct ( decide (p = x)). subst. destruct o. simpl in *. inversion H. eauto. simpl in *. destruct o. simpl in *. inversion H. simpl in *. apply IHm in H. eauto.
-
-            +induction m. simpl in *. auto. simpl in *. destruct a. simpl in *. specialize (H p). rewrite eq_refl in H. destruct o. simpl in *. inversion H. simpl in *. apply IHm. simpl in *. intros. Admitted.
-  
-    Lemma beq_correct:
-      forall m1 m2,
-      beq m1 m2 = true <->
-      (forall (x: elt),
-       match get x m1, get x m2 with
-       | None, None => True
-       | Some y1, Some y2 => beqA y1 y2 = true
-       | _, _ => False
-       end).
     Proof. Admitted.
 
 
-
-
-
-
-
-           
+    Lemma beq_correct: forall m1 m2, beq m1 m2 = true <-> (forall (x: elt),
+                                                              match get x m1, get x m2 with
+                                                                           | None, None => True
+                                                                           | Some y1, Some y2 => beqA y1 y2 = true
+                                                                           | _, _ => False
+                                                                                       end).
+Proof. Admitted.
   End BOOLEAN_EQUALITY.
-(*
-  Fixpoint prev_append (i j: pc) {struct i} : positive :=
-    match i with
-      | xH => j
-      | xI i' => prev_append i' (xI j)
-      | xO i' => prev_append i' (xO j)
-    end.
-
-  Definition prev (i: positive) : positive :=
-    prev_append i xH.
-
-  Lemma prev_append_prev i j:
-    prev (prev_append i j) = prev_append j i.
-Proof.
-
-  Lemma prev_involutive i :
-    prev (prev i) = i.
-  Proof (prev_append_prev i xH).
-
-  Lemma prev_append_inj i j j' :
-    prev_append i j = prev_append i j' -> j = j'.
-Proof.
- *)
-  (*
-    Fixpoint xmap (A B : Type) (f : pc -> A -> B) (m : t A) (i : positive)
-             {struct m} : t B :=
-      match m with
-      | nil => nil
-      | cons hd tl => cons (f (fst hd) (snd hd)) xmap f tl end.
 
 
-      l o r => Node (xmap f l (xO i))
-                           (match o with None => None | Some x => Some (f (prev i) x) end)
-                           (xmap f r (xI i))
-      end.
 
-  Definition map (A B : Type) (f : positive -> A -> B) m := xmap f m xH.
+Print t.
 
-    Lemma xgmap:
-      forall (A B: Type) (f: positive -> A -> B) (i j : positive) (m: t A),
-      get i (xmap f m j) = option_map (f (prev (prev_append i j))) (get i m).
-Proof.
-
-  Theorem gmap:
-    forall (A B: Type) (f: positive -> A -> B) (i: positive) (m: t A),
-    get i (map f m) = option_map (f i) (get i m).
-Proof.
-   *)
-
-  Print t.
-
-  Print option_map.
-
-
-  Print t.
-
-  
-  Definition map1_single A B (f : A -> B) (item:(pc * option A)) : (pc*option B):=
-    match item with
-      | (first, second) => (first, option_map f second)
-    end. Print t.
-  Fixpoint map1 (A B: Type) (f: A -> B) (m: t A) {struct m} : t B :=
+  Fixpoint map (A B: Type) (f: local_id -> A -> B) m : t B :=
     match m with
     | nil => nil
-    | hd :: tl => (map1_single f hd) :: (map1 f tl)
+    | (key, Some item) :: tl => (key, Some (f key item)) :: map f tl
+    | (key, None) :: tl => (key, None) :: map f tl
     end.
-(*
+ 
+
+  Fixpoint map1 (A B: Type) (f: A -> B) (m: t A) : t B :=
+    match m with
+    | nil => nil
+    | (key, None) :: tl => (key, None) :: map1 f tl
+    | (key, Some a) :: tl => (key, Some (f a)) :: map1 f tl
+    end.
+  
+      
+
+  Theorem gmap: forall (A B: Type) (f: local_id -> A -> B) (i: local_id) (m: t A),
+      get i (map f m) = option_map (f i) (get i m).
+  Proof. intros. induction m. simpl in *. auto. simpl in *. destruct a. simpl in *. destruct o. simpl in *. destruct (elt_eq e i). subst. eauto. simpl in *. eauto. simpl in *. destruct ( elt_eq e i). subst. simpl in *. eauto. eauto. Qed.
+
+
+
+
   Theorem gmap1:
     forall (A B: Type) (f: A -> B) (i: elt) (m: t A),
-    get i (map1 f m) = option_map f (get i m).
-Proof.
+      get i (map1 f m) = option_map f (get i m).
+  Proof. induction m. simpl in *. auto. simpl in *. destruct a. simpl in *. destruct o. simpl in *. destruct (elt_eq e i). subst. simpl in *. auto. eauto. simpl in *.  destruct ( elt_eq e i). subst. simpl in *. eauto. eauto. Qed.
 
-  Definition Node' (A: Type) (l: t A) (x: option A) (r: t A): t A :=
-    match l, x, r with
-    | Leaf, None, Leaf => Leaf
-    | _, _, _ => Node l x r
-    end.
 
-  Lemma gnode':
-    forall (A: Type) (l r: t A) (x: option A) (i: positive),
-    get i (Node' l x r) = get i (Node l x r).
-Proof.
 
-  Fixpoint filter1 (A: Type) (pred: A -> bool) (m: t A) {struct m} : t A :=
-    match m with
-    | Leaf => Leaf
-    | Node l o r =>
-        let o' := match o with None => None | Some x => if pred x then o else None end in
-        Node' (filter1 pred l) o' (filter1 pred r)
-    end.
 
-  Theorem gfilter1:
-    forall (A: Type) (pred: A -> bool) (i: elt) (m: t A),
-    get i (filter1 pred m) =
-    match get i m with None => None | Some x => if pred x then Some x else None end.
-Proof.
-   *)
-  (*
+
   Section COMBINE.
 
-  Variables A B C: Type.
-  Variable f: option A -> option B -> option C.
-  Hypothesis f_none_none: f None None = None.
+    Variables A B C: Type.
+    Variable f: option A -> option B -> option C.
+    Hypothesis f_none_none: f None None = None.
+
+Print t.
+
+Print tree.
 
   Fixpoint xcombine_l (m : t A) {struct m} : t C :=
-      match m with
-      | Leaf => Leaf
-      | Node l o r => Node' (xcombine_l l) (f o None) (xcombine_l r)
+    match m with
+    | nil => nil
+               | (key, val) :: tl => (key, (f val None)) :: xcombine_l tl
+    (*  | Leaf => Leaf
+      | Node l o r => Node' (xcombine_l l) (f o None) (xcombine_l r)*)
       end.
+
 
   Lemma xgcombine_l :
-          forall (m: t A) (i : positive),
+          forall m i,
           get i (xcombine_l m) = f (get i m) None.
 Proof.
+      induction m; intros; simpl; symmetry; eauto. destruct a. simpl in *. remember ( elt_eq e i). destruct s. simpl in *. eauto. symmetry. eauto. Qed.
 
   Fixpoint xcombine_r (m : t B) {struct m} : t C :=
-      match m with
-      | Leaf => Leaf
-      | Node l o r => Node' (xcombine_r l) (f None o) (xcombine_r r)
+    match m with
+    | nil => nil
+    | (key, val) :: tl => (key, (f None val)) :: xcombine_r tl
       end.
+
 
   Lemma xgcombine_r :
-          forall (m: t B) (i : positive),
+          forall m i,
           get i (xcombine_r m) = f None (get i m).
 Proof.
+      induction m; intros; simpl; symmetry; eauto. destruct a. simpl in *. remember ( elt_eq e i). destruct s. simpl in *. eauto. symmetry. eauto. Qed.
 
-  Fixpoint combine (m1: t A) (m2: t B) {struct m1} : t C :=
-    match m1 with
-    | Leaf => xcombine_r m2
-    | Node l1 o1 r1 =>
-        match m2 with
-        | Leaf => xcombine_l m1
-        | Node l2 o2 r2 => Node' (combine l1 l2) (f o1 o2) (combine r1 r2)
-        end
-    end.
 
-  Theorem gcombine:
-      forall (m1: t A) (m2: t B) (i: positive),
+
+Fixpoint combine (l1: t A) (l2: t B) :=
+  match l1 with
+  | nil => xcombine_r l2
+  | (a, b) :: tl => match get a l2 with
+                       | None => (a, f b None) :: combine tl (remove a l2)
+                       | Some res => (a, f b (Some res)) :: combine tl (remove a l2)
+                       end
+                         
+                       
+  end.
+
+
+
+Theorem gcombine:
+      forall m1 m2 i,
       get i (combine m1 m2) = f (get i m1) (get i m2).
-Proof.
+Proof. 
+ Admitted.
 
-  End COMBINE.
 
-  Lemma xcombine_lr :
-    forall (A B: Type) (f g : option A -> option A -> option B) (m : t A),
-    (forall (i j : option A), f i j = g j i) ->
-    xcombine_l f m = xcombine_r g m.
-Proof.
 
-  Theorem combine_commut:
-    forall (A B: Type) (f g: option A -> option A -> option B),
-    (forall (i j: option A), f i j = g j i) ->
-    forall (m1 m2: t A),
-    combine f m1 m2 = combine g m2 m1.
-Proof.
+End COMBINE.
+     
 
-    Fixpoint xelements (A : Type) (m : t A) (i : positive)
-                       (k: list (positive * A)) {struct m}
-                       : list (positive * A) :=
-      match m with
-      | Leaf => k
-      | Node l None r =>
-          xelements l (xO i) (xelements r (xI i) k)
-      | Node l (Some x) r =>
-          xelements l (xO i)
-            ((prev i, x) :: xelements r (xI i) k)
-      end.
-
-  Definition elements (A: Type) (m : t A) := xelements m xH nil.
-
-  Remark xelements_append:
-    forall A (m: t A) i k1 k2,
-    xelements m i (k1 ++ k2) = xelements m i k1 ++ k2.
-Proof.
-
-  Remark xelements_leaf:
-    forall A i, xelements (@Leaf A) i nil = nil.
-Proof.
-
-  Remark xelements_node:
-    forall A (m1: t A) o (m2: t A) i,
-    xelements (Node m1 o m2) i nil =
-       xelements m1 (xO i) nil
-    ++ match o with None => nil | Some v => (prev i, v) :: nil end
-    ++ xelements m2 (xI i) nil.
-Proof.
-
-    Lemma xelements_incl:
-      forall (A: Type) (m: t A) (i : positive) k x,
-      In x k -> In x (xelements m i k).
-Proof.
-
-    Lemma xelements_correct:
-      forall (A: Type) (m: t A) (i j : positive) (v: A) k,
-      get i m = Some v -> In (prev (prev_append i j), v) (xelements m j k).
-Proof.
-
-  Theorem elements_correct:
-    forall (A: Type) (m: t A) (i: positive) (v: A),
-    get i m = Some v -> In (i, v) (elements m).
-Proof.
-
-  Lemma in_xelements:
-    forall (A: Type) (m: t A) (i k: positive) (v: A) ,
-    In (k, v) (xelements m i nil) ->
-    exists j, k = prev (prev_append j i) /\ get j m = Some v.
-Proof.
+  Fixpoint elements A (m : t A) : (list (local_id * A)) :=
+    match m with
+    | nil => nil
+    | (key, Some item) :: tl => (key, item) :: elements tl
+    | _ :: tl => elements tl
+    end.
+  
+                                                    
+  Theorem elements_correct: forall (A: Type) (m: t A) (i: local_id) (v: A),
+      get i m = Some v -> In (i, v) (elements m).
+  Proof. induction m. simpl in *. intros. inversion H.
+         simpl in *. destruct a. simpl in *. intros. destruct (elt_eq e i). subst. simpl in *. left. auto. simpl in *. destruct o. simpl in *. subst. right. apply IHm. auto. apply IHm. apply H. Qed.
+  
 
   Theorem elements_complete:
-    forall (A: Type) (m: t A) (i: positive) (v: A),
-    In (i, v) (elements m) -> get i m = Some v.
-Proof.
+    forall (A: Type) (m: t A) (i: local_id) (v: A),
+      In (i, v) (elements m) -> get i m = Some v.
+  Proof. induction m. intros. simpl in *. inversion H. intros. simpl in *.   destruct a.
+destruct ( elt_eq e i).
 
-  Definition xkeys (A: Type) (m: t A) (i: positive) :=
-    List.map (@fst positive A) (xelements m i nil).
 
-  Remark xkeys_leaf:
-    forall A i, xkeys (@Leaf A) i = nil.
-Proof.
 
-  Remark xkeys_node:
-    forall A (m1: t A) o (m2: t A) i,
-    xkeys (Node m1 o m2) i =
-       xkeys m1 (xO i)
-    ++ match o with None => nil | Some v => prev i :: nil end
-    ++ xkeys m2 (xI i).
-Proof.
+  Admitted.
 
-  Lemma in_xkeys:
-    forall (A: Type) (m: t A) (i k: positive),
-    In k (xkeys m i) ->
-    (exists j, k = prev (prev_append j i)).
-Proof.
 
+
+  Definition xkeys (A: Type) (m: t A) (i: local_id) :=
+    List.map fst m.
+
+Print list_norepet.
   Lemma xelements_keys_norepet:
-    forall (A: Type) (m: t A) (i: positive),
-    list_norepet (xkeys m i).
-Proof.
+    forall (A: Type) (m: t A) (i: local_id),
+      list_norepet (xkeys m i).
+Proof. intros. induction m. simpl in *. constructor. simpl in *. destruct a. simpl in *. constructor. simpl in *. Admitted.
 
-  Theorem elements_keys_norepet:
-    forall (A: Type) (m: t A),
-    list_norepet (List.map (@fst elt A) (elements m)).
-Proof.
 
-  Remark xelements_empty:
-    forall (A: Type) (m: t A) i, (forall i, get i m = None) -> xelements m i nil = nil.
-Proof.
+Theorem elements_keys_norepet:
+  forall (A: Type) (m: t A),
+    list_norepet (List.map fst (elements m)). Proof. Admitted.
 
-  Theorem elements_canonical_order':
-    forall (A B: Type) (R: A -> B -> Prop) (m: t A) (n: t B),
-    (forall i, option_rel R (get i m) (get i n)) ->
-    list_forall2
-      (fun i_x i_y => fst i_x = fst i_y /\ R (snd i_x) (snd i_y))
-      (elements m) (elements n).
-Proof.
 
-  Theorem elements_canonical_order:
-    forall (A B: Type) (R: A -> B -> Prop) (m: t A) (n: t B),
-    (forall i x, get i m = Some x -> exists y, get i n = Some y /\ R x y) ->
-    (forall i y, get i n = Some y -> exists x, get i m = Some x /\ R x y) ->
-    list_forall2
-      (fun i_x i_y => fst i_x = fst i_y /\ R (snd i_x) (snd i_y))
-      (elements m) (elements n).
-Proof.
 
-  Theorem elements_extensional:
-    forall (A: Type) (m n: t A),
+Theorem elements_extensional:
+  forall (A: Type) (m n: t A),
     (forall i, get i m = get i n) ->
     elements m = elements n.
-Proof.
+Proof. Admitted.
 
-  Lemma xelements_remove:
-    forall (A: Type) v (m: t A) i j,
+Theorem elements_remove:
+  forall (A: Type) i v (m: t A),
     get i m = Some v ->
-    exists l1 l2,
-    xelements m j nil = l1 ++ (prev (prev_append i j), v) :: l2
-    /\ xelements (remove i m) j nil = l1 ++ l2.
-Proof.
+    exists l1 l2, elements m = l1 ++ (i, v) :: l2 /\ elements (remove i m) = l1 ++ l2.
+Proof. intros. Admitted.
 
-  Theorem elements_remove:
-    forall (A: Type) i v (m: t A),
-    get i m = Some v ->
-    exists l1 l2, elements m = l1 ++ (i,v) :: l2 /\ elements (remove i m) = l1 ++ l2.
-Proof.
 
-  Fixpoint xfold (A B: Type) (f: B -> positive -> A -> B)
-                 (i: positive) (m: t A) (v: B) {struct m} : B :=
-    match m with
-    | Leaf => v
-    | Node l None r =>
-        let v1 := xfold f (xO i) l v in
-        xfold f (xI i) r v1
-    | Node l (Some x) r =>
-        let v1 := xfold f (xO i) l v in
-        let v2 := f v1 (prev i) x in
-        xfold f (xI i) r v2
-    end.
+Fixpoint fold1 (A B: Type) (f: B -> A -> B) (m: t A) (v: B) : B :=
+  match m with
+  | nil => v
+  | (key, Some item) :: tl => fold1 f tl (f v item)
+  | (key, None) :: tl => fold1 f tl v
+  end.
 
-  Definition fold (A B : Type) (f: B -> positive -> A -> B) (m: t A) (v: B) :=
-    xfold f xH m v.
+Fixpoint fold (A B: Type) (f: B -> local_id -> A -> B) (m: t A) (v: B) : B :=
+  match m with
+  | nil => v
+  | (key, Some item) :: tl => fold f tl (f v key item)
+  | (key, None) :: tl => fold f tl v
+  end.
 
-  Lemma xfold_xelements:
-    forall (A B: Type) (f: B -> positive -> A -> B) m i v l,
-    List.fold_left (fun a p => f a (fst p) (snd p)) l (xfold f i m v) =
-    List.fold_left (fun a p => f a (fst p) (snd p)) (xelements m i l) v.
-Proof.
 
-  Theorem fold_spec:
-    forall (A B: Type) (f: B -> positive -> A -> B) (v: B) (m: t A),
+Theorem fold_spec:
+  forall (A B: Type) (f: B -> local_id -> A -> B) (v: B) (m: t A),
     fold f m v =
     List.fold_left (fun a p => f a (fst p) (snd p)) (elements m) v.
-Proof.
+Proof. induction m. simpl in *. auto.
+       simpl in *. destruct a. simpl in *. destruct o. simpl in *. eauto. Admitted.
 
-  Fixpoint fold1 (A B: Type) (f: B -> A -> B) (m: t A) (v: B) {struct m} : B :=
-    match m with
-    | Leaf => v
-    | Node l None r =>
-        let v1 := fold1 f l v in
-        fold1 f r v1
-    | Node l (Some x) r =>
-        let v1 := fold1 f l v in
-        let v2 := f v1 x in
-        fold1 f r v2
-    end.
-
-  Lemma fold1_xelements:
-    forall (A B: Type) (f: B -> A -> B) m i v l,
-    List.fold_left (fun a p => f a (snd p)) l (fold1 f m v) =
-    List.fold_left (fun a p => f a (snd p)) (xelements m i l) v.
-Proof.
-
-  Theorem fold1_spec:
-    forall (A B: Type) (f: B -> A -> B) (v: B) (m: t A),
+Theorem fold1_spec:
+  forall (A B: Type) (f: B -> A -> B) (v: B) (m: t A),
     fold1 f m v =
     List.fold_left (fun a p => f a (snd p)) (elements m) v.
-Proof.
-*)
-End PList.
+  Proof. Admitted.
+End lidTree.
 
+  
+Module lidMap <: MAP.
+  Definition elt := local_id.
+  Definition elt_eq := loc_id_eq.
 
-Module PMap.
-  Definition elt := pc.
-  Definition pc_comp (A B:pc) : bool := decide (A = B).
+  Definition t (A : Type) : Type := (A * lidTree.t A)%type.
 
-  Definition elt_eq := pc_comp.
+  Definition init (A : Type) (x: A) :=
+    (x, lidTree.empty A).
 
-  Definition t (A : Type) : Type := (A * PList.t A)%type.
-
-  Definition init (A : Type) (x : A) :=
-    (x, PList.empty A).
-
-  Definition get (A : Type) (i : pc) (m : t A) :=
-    match PList.get i (snd m) with
+  Definition get (A: Type) (i: local_id) (m: t A) :=
+    match lidTree.get i (snd m) with
     | Some x => x
     | None => fst m
     end.
 
-  Definition set (A : Type) (i : pc) (x : A) (m : t A) :=
-    (fst m, PList.set i x (snd m)).
 
-  Theorem gi:
-    forall (A: Type) (i: pc) (x: A), get A i (init A x) = x.
-Proof.
-  intros. unfold init. simpl in *. unfold get. simpl in *. eauto. Qed.
-Hint Resolve gi.
+  Definition set (A: Type) (i : local_id) (x : A) (m : t A) :=
+    (fst m, lidTree.set i x (snd m)).
+
+
+  Theorem gi: forall (A: Type) (i: local_id) (x: A), get i (init x) = x.
+  Proof. intros. unfold init. unfold get. rewrite lidTree.gempty. simpl in *. auto. Qed.
+
+
   Theorem gss:
-    forall (A: Type) (i: pc) (x: A) (m: t A), get A i (set A i x m) = x.
-Proof.
-  intros. induction m. simpl in *. unfold set. simpl in *. unfold get. simpl in *. SearchAbout PList.get.
-rewrite PList.gss. eauto. Qed.
+    forall (A: Type) (i: local_id) (x: A) (m: t A), get i (set i x m) = x.
+  Proof. intros. unfold get. unfold set. simpl in *. rewrite lidTree.gss. auto. Qed.
 
 
-            
   Theorem gso:
-    forall (A: Type) (i j: pc) (x: A) (m: t A),
-    i <> j -> get A i (set A j x m) = get A i m.
-Proof. intros. induction m. simpl in *. simpl in *. unfold set. simpl in *. unfold get. simpl in *. remember ( PList.get i (PList.set j x b) ). eapply PList.gso in H. rewrite <- Heqo in H. clear Heqo. rewrite H. auto. Qed.
-  
+    forall (A: Type) (i j: local_id) (x: A) (m: t A),
+      i <> j -> get i (set j x m) = get i m.
+  Proof. intros. unfold get. unfold set. simpl in *. rewrite lidTree.gso; eauto.
+  Qed.
+
   Theorem gsspec:
-    forall (A: Type) (i j: pc) (x: A) (m: t A),
-    get A i (set A j x m) = if elt_eq i j then x else get A i m.
-Proof.
-intros. unfold get, set. simpl in *. Admitted.
+    forall (A: Type) (i j: local_id) (x: A) (m: t A),
+      get i (set j x m) = if elt_eq i j then x else get i m.
+  Proof. intros.  destruct (elt_eq i j). subst. apply gss. rewrite gso. auto. auto. Qed.
 
 
 
-  
   Theorem gsident:
-    forall (A: Type) (i j: pc) (m: t A),
-    get A j (set A i (get A i m) m) = get A j m.
-Proof.
-  Proof. intros.
-  Admitted.
+    forall (A: Type) (i j: local_id) (m: t A),
+      get j (set i (get i m) m) = get j m.
+  Proof. intros. destruct ( elt_eq i j). simpl in *. subst. rewrite gss. auto. rewrite gso; eauto. Qed.
 
-  
-  Definition map (A B : Type) (f : A -> B) (m : t A) : t B :=
-    (f (fst m),PList.map1 f (snd m)).
+
+  Definition map (A B: Type) (f: A -> B) (m: t A) : t B := (f (fst m), lidTree.map1 f (snd m)).
+
+
+
+
 
   Theorem gmap:
-    forall (A B: Type) (f: A -> B) (i: pc) (m: t A),
-    get B i (map A B f m) = f(get A i m).
-Proof.
-  intros. induction m; simpl in *. unfold map. simpl in *. unfold get. simpl in *. Admitted.
+    forall (A B: Type) (f: A -> B) (i: local_id) (m: t A),
+      get i (map f m) = f (get i m).
+  Proof. intros. unfold map. unfold get. simpl in *. rewrite lidTree.gmap1. unfold option_map.
+         destruct (lidTree.get i (snd m)); eauto. Qed.
 
 
-Print elt.
-
-  
   Theorem set2:
     forall (A: Type) (i: elt) (x y: A) (m: t A),
-    set A i y (set A i x m) = set A i y m.
-Proof.
-Admitted.
-End PMap.
+      set i y (set i x m) = set i y m.
+  Proof.
+    intros. unfold set. simpl in *. decEq. Admitted.
+End lidMap.
+  
+
+
+
+Notation "a # b" := (lidTree.get b a) (at level 1).
+Notation "a ## b" := (lidMap.get b a) (at level 1).
 
 
 
 
-Notation "a ! b" := (PList.get b a) (at level 1).
-Notation "a !! b" := (PMap.get b a) (at level 1).
+
+(*********)
 
 
-
-Module Type SEMILATTICE.
-
-  Parameter t: Type.
-  Parameter eq: t -> t -> Prop.
-  Axiom eq_refl: forall x, eq x x.
-  Axiom eq_sym: forall x y, eq x y -> eq y x.
-  Axiom eq_trans: forall x y z, eq x y -> eq y z -> eq x z.
-  Parameter beq: t -> t -> bool.
-  Axiom beq_correct: forall x y, beq x y = true -> eq x y.
-  Parameter ge: t -> t -> Prop.
-  Axiom ge_refl: forall x y, eq x y -> ge x y.
-  Axiom ge_trans: forall x y z, ge x y -> ge y z -> ge x z.
-  Parameter bot: t.
-  Axiom ge_bot: forall x, ge x bot.
-  Parameter lub: t -> t -> t.
-  Axiom ge_lub_left: forall x y, ge (lub x y) x.
-  Axiom ge_lub_right: forall x y, ge (lub x y) y.
-
-End SEMILATTICE.
-
-
-Module Type DATAFLOW_SOLVER.
-
-  Declare Module L: SEMILATTICE.
-
-  Parameter fixpoint:
-    forall {A: Type} (code: PList.t A) (successors: A -> list pc)
-           (transf: pc -> L.t -> L.t)
-           (ep: pc) (ev: L.t),
-    option (PMap.t L.t).
-Print PList.get.
-Print SEMILATTICE.
-
-
-Print state.
-
-
-Module Type NODE_SET.
-
-  Parameter t: Type.
-  Parameter empty: t.
-  Parameter add: pc -> t -> t.
-  Parameter pick: t -> option (pc * t).
-  Parameter all_nodes: forall {A: Type}, PList.t A -> t.
-
-  Parameter In: pc -> t -> Prop.
-  Axiom empty_spec:
-    forall n, ~In n empty.
-  Axiom add_spec:
-    forall n n' s, In n' (add n s) <-> n = n' \/ In n' s.
-  Axiom pick_none:
-    forall s n, pick s = None -> ~In n s.
-  Axiom pick_some:
-    forall s n s', pick s = Some(n, s') ->
-    forall n', In n' s <-> n = n' \/ In n' s'.
-  Axiom all_nodes_spec:
-    forall A (code: PList.t A) n instr,
-    code!n = Some instr -> In n (all_nodes code).
-
-End NODE_SET.
-
-
-
-
-Module Dataflow_Solver (LAT: SEMILATTICE) (NS: NODE_SET)  := LAT.
-
-
-Section Kildall.
-
-Context {A: Type}.
-Variable code: PList.t A.
-Variable successors: A -> list pc.
-Variable transf: pc -> L.t -> L.t.
-
-
-
-Record state : Type :=
-  mkstate { aval: PList.t L.t; worklist: list A; visited: positive -> Prop }.
-
-Definition abstr_value (n: pc) (s: state) : L.t :=
-  match s.(aval)!n with
-  | None => L.bot
-  | Some v => v
-  end.
-
-(*
-Definition propagate_succ (s: state) (out: L.t) (n: positive) :=
-  match s.(aval)!n with
-  | None =>
-      {| aval := PTree.set n out s.(aval);
-         worklist := NS.add n s.(worklist);
-         visited := fun p => p = n \/ s.(visited) p |}
-  | Some oldl =>
-      let newl := L.lub oldl out in
-      if L.beq oldl newl
-      then s
-      else {| aval := PTree.set n newl s.(aval);
-              worklist := NS.add n s.(worklist);
-              visited := fun p => p = n \/ s.(visited) p |}
-  end.
-
-propagate_succ_list corresponds, in the pseudocode, to the for loop iterating over all successors.
-
-Fixpoint propagate_succ_list (s: state) (out: L.t) (succs: list positive)
-                             {struct succs} : state :=
-  match succs with
-  | nil => s
-  | n :: rem => propagate_succ_list (propagate_succ s out n) out rem
-  end.
-
-step corresponds to the body of the outer while loop in the pseudocode.
-
-Definition step (s: state) : PMap.t L.t + state :=
-  match NS.pick s.(worklist) with
-  | None =>
-      inl _ (L.bot, s.(aval))
-  | Some(n, rem) =>
-      match code!n with
-      | None =>
-          inr _ {| aval := s.(aval); worklist := rem; visited := s.(visited) |}
-      | Some instr =>
-          inr _ (propagate_succ_list
-                  {| aval := s.(aval); worklist := rem; visited := s.(visited) |}
-                  (transf n (abstr_value n s))
-                  (successors instr))
-      end
-  end.
-
-The whole fixpoint computation is the iteration of step from an initial state.
-
-Definition fixpoint_from (start: state) : option (PMap.t L.t) :=
-  PrimIter.iterate _ _ step start.
- *)
-
-
-
-(*Definition start_state (enode: positive) (eval: L.t) :=
-  {| aval := PTree.set enode eval (PTree.empty L.t);
-     worklist := NS.add enode NS.empty;
-     visited := fun n => n = enode |}.
-
-Definition fixpoint (enode: positive) (eval: L.t) :=
-  fixpoint_from (start_state enode eval).
- *)
-
-
-
-(*Record good_state (st: state) : Prop := {
-  gs_stable: forall n,
-    st.(visited) n ->
-    NS.In n st.(worklist) \/
-    (forall i s,
-     code!n = Some i -> In s (successors i) ->
-     optge st.(aval)!s (Some (transf n (abstr_value n st))));
-  gs_defined: forall n v,
-    st.(aval)!n = Some v -> st.(visited) n
-}.
-
- *)
-(*
-
-Lemma step_state_good:
-  forall st pc rem instr,
-  NS.pick st.(worklist) = Some (pc, rem) ->
-  code!pc = Some instr ->
-  good_state st ->
-  good_state (propagate_succ_list (mkstate st.(aval) rem st.(visited))
-                                  (transf pc (abstr_value pc st))
-                                  (successors instr)).
-Proof.
- *)
-
-
-(*Lemma step_state_good_2:
-  forall st pc rem,
-  good_state st ->
-  NS.pick (worklist st) = Some (pc, rem) ->
-  code!pc = None ->
-  good_state (mkstate st.(aval) rem st.(visited)).
-Proof.
-
-Lemma steps_state_good:
-  forall st1 st2, steps st1 st2 -> good_state st1 -> good_state st2.
-Proof.
- *)
-
-(*Lemma start_state_good:
-  forall enode eval, good_state (start_state enode eval).
-Proof.
-  intros. unfold start_state; constructor; simpl; intros.
-- subst n. rewrite NS.add_spec; auto.
-- rewrite PTree.gsspec in H. rewrite PTree.gempty in H.
-  destruct (peq n enode). auto. discriminate.
-Qed.
-
-Lemma start_state_nodeset_good:
-  forall enodes, good_state (start_state_nodeset enodes).
-Proof.
-  intros. unfold start_state_nodeset; constructor; simpl; intros.
-- left. auto.
-- rewrite PTree.gempty in H. congruence.
-Qed.
-
-Lemma start_state_allnodes_good:
-  good_state start_state_allnodes.
-Proof.
-  unfold start_state_allnodes; constructor; simpl; intros.
-- destruct H as [instr CODE]. left. eapply NS.all_nodes_spec; eauto.
-- rewrite PTree.gempty in H. congruence.
-Qed.
-*)*)
