src/coq/optimisations/Kildall/lattice.v
@@ -1,0 +1,565 @@
+Require Import Coqlib.
+Require Import  Vellvm.Ollvm_ast Vellvm.Classes Vellvm.Util Vellvm.CFGProp Vellvm.CFG.
+Require Import Vellvm.optimisations.maps.
+Require Import FSets.
+
+
+Module Type SEMILATTICE.
+
+
+  Parameter t: Type.
+  Parameter eq: t -> t -> Prop.
+  Axiom eq_refl: forall x, eq x x.
+  Axiom eq_sym: forall x y, eq x y -> eq y x.
+  Axiom eq_trans: forall x y z, eq x y -> eq y z -> eq x z.
+  Parameter beq: t -> t -> bool.
+  Axiom beq_correct: forall x y, beq x y = true -> eq x y.
+  Parameter ge: t -> t -> Prop.
+  Axiom ge_refl: forall x y, eq x y -> ge x y.
+  Axiom ge_trans: forall x y z, ge x y -> ge y z -> ge x z.
+  Parameter bot: t.
+  Axiom ge_bot: forall x, ge x bot.
+  Parameter lub: t -> t -> t.
+  Axiom ge_lub_left: forall x y, ge (lub x y) x.
+  Axiom ge_lub_right: forall x y, ge (lub x y) y.
+
+End SEMILATTICE.
+
+
+Module Type SEMILATTICE_WITH_TOP.
+
+  Include SEMILATTICE.
+  Parameter top: t.
+  Axiom ge_top: forall x, ge top x.
+
+End SEMILATTICE_WITH_TOP.
+
+
+
+Module LPMap1(L: SEMILATTICE) <: SEMILATTICE.
+
+  Definition t := PCTree.t L.t.
+
+  Definition get (p: pc) (x: t) : L.t :=
+  match x!p with None => L.bot | Some x => x end.
+
+
+  Definition set (p: pc) (v: L.t) (x: t) : t :=
+  if L.beq v L.bot
+  then PCTree.remove p x
+  else PCTree.set p v x.
+
+
+  
+  Lemma gsspec:
+  forall p v x q,
+  L.eq (get q (set p v x)) (if PC.eqb q p then v else get q x).
+  Proof.
+  intros. unfold set, get.
+  destruct (L.beq v L.bot) eqn:EBOT.
+  rewrite PCTree.grspec. destruct ( PCTree.elt_eq q p). subst. destruct ( PC.eqb p p) eqn:?. unfold PC.eqb in *.
+  destruct ( PC.eq_dec p p). eapply L.eq_sym. eapply L.beq_correct. eauto. contradiction n; eauto.
+  unfold PC.eqb in *. simpl in *. destruct ( PC.eq_dec p p). inversion Heqb. contradiction n; eauto.
+  apply L.eq_sym. simpl in *. unfold PC.eqb. simpl in *.
+destruct (PC.eq_dec q p). subst. contradiction n; eauto. apply L.eq_refl.
+  rewrite PCTree.gsspec. unfold PCTree.elt_eq. simpl in *.
+  destruct (PCTree.pc_eq q p). destruct ( PC.eqb q p) eqn:?. apply L.eq_refl.  subst.
+unfold PC.eqb in *. destruct ( PC.eq_dec p p). inversion Heqb. contradiction n; eauto. 
+destruct ( PC.eqb q p ) eqn:?. unfold PC.eqb in *. simpl in *.
+destruct ( PC.eq_dec q p). subst. contradiction n; eauto. inversion Heqb. eapply L.eq_refl.
+  Qed.
+
+
+
+
+Definition eq (x y: t) : Prop :=
+  forall p, L.eq (get p x) (get p y).
+
+Lemma eq_refl: forall x, eq x x.
+Proof. unfold eq; intros; apply L.eq_refl. Qed.
+
+
+Lemma eq_sym: forall x y, eq x y -> eq y x.
+Proof.
+  unfold eq; intros. apply L.eq_sym; auto.
+Qed.
+
+Lemma eq_trans: forall x y z, eq x y -> eq y z -> eq x z.
+Proof.
+  unfold eq; intros. eapply L.eq_trans; eauto.
+Qed.
+
+Definition beq (x y: t) : bool := PCTree.beq L.beq x y.
+
+Lemma beq_correct: forall x y, beq x y = true -> eq x y.
+Proof.
+  unfold beq; intros; red; intros. unfold get.
+  rewrite PCTree.beq_correct in H. specialize (H p).
+  destruct (x!p); destruct (y!p); intuition.
+  apply L.beq_correct; auto.
+  apply L.eq_refl.
+Qed.
+
+Definition ge (x y: t) : Prop :=
+  forall p, L.ge (get p x) (get p y).
+
+Lemma ge_refl: forall x y, eq x y -> ge x y.
+Proof.
+  unfold ge, eq; intros. apply L.ge_refl. auto.
+Qed.
+
+Lemma ge_trans: forall x y z, ge x y -> ge y z -> ge x z.
+Proof.
+  unfold ge; intros. apply L.ge_trans with (get p y); auto.
+Qed.
+
+Definition bot : t := PCTree.empty _.
+
+Lemma get_bot: forall p, get p bot = L.bot.
+Proof.
+  unfold bot, get; intros; simpl. auto.
+Qed.
+
+Lemma ge_bot: forall x, ge x bot.
+Proof.
+  unfold ge; intros. rewrite get_bot. apply L.ge_bot.
+Qed.
+
+
+Section COMBINE.
+
+  Variable f: option L.t -> option L.t -> option L.t.
+Hypothesis f_none_none: f None None = None.
+
+Definition opt_eq (ox oy: option L.t) : Prop :=
+  match ox, oy with
+  | None, None => True
+  | Some x, Some y => L.eq x y
+  | _, _ => False
+  end.
+
+Lemma opt_eq_refl: forall ox, opt_eq ox ox.
+Proof.
+  intros. unfold opt_eq. destruct ox. apply L.eq_refl. auto.
+Qed.
+
+Lemma opt_eq_sym: forall ox oy, opt_eq ox oy -> opt_eq oy ox.
+Proof.
+  unfold opt_eq. destruct ox; destruct oy; auto. apply L.eq_sym.
+Qed.
+
+Lemma opt_eq_trans: forall ox oy oz, opt_eq ox oy -> opt_eq oy oz -> opt_eq ox oz.
+Proof.
+  unfold opt_eq. destruct ox; destruct oy; destruct oz; intuition.
+  eapply L.eq_trans; eauto.
+Qed.
+
+Definition opt_beq (ox oy: option L.t) : bool :=
+  match ox, oy with
+  | None, None => true
+  | Some x, Some y => L.beq x y
+  | _, _ => false
+  end.
+
+Lemma opt_beq_correct:
+  forall ox oy, opt_beq ox oy = true -> opt_eq ox oy.
+Proof.
+  unfold opt_beq, opt_eq. destruct ox; destruct oy; try congruence.
+  intros. apply L.beq_correct; auto.
+  auto.
+Qed.
+
+Definition tree_eq (m1 m2: PCTree.t L.t) : Prop :=
+  forall i, opt_eq (PCTree.get i m1) (PCTree.get i m2).
+
+Lemma tree_eq_refl: forall m, tree_eq m m.
+Proof.
+intros; red; intros; apply opt_eq_refl. Qed.
+
+Lemma tree_eq_sym: forall m1 m2, tree_eq m1 m2 -> tree_eq m2 m1.
+Proof.
+intros; red; intros; apply opt_eq_sym; auto. Qed.
+
+Lemma tree_eq_trans: forall m1 m2 m3, tree_eq m1 m2 -> tree_eq m2 m3 -> tree_eq m1 m3.
+Proof.
+intros; red; intros; apply opt_eq_trans with (PCTree.get i m2); auto. Qed.
+
+End COMBINE.
+
+
+Print t.
+Print PCTree.combine.
+
+Definition lub (x y: t) : t :=
+  PCTree.combine
+    (fun a b =>
+       match a, b with
+       | Some u, Some v => Some (L.lub u v)
+       | None, _ => b
+       | _, None => a
+       end)
+    x y.
+
+
+Lemma ge_lub_left:
+  forall x y, ge (lub x y) x.
+Proof.
+  unfold ge, lub; intros.
+  eapply L.ge_trans. apply L.ge_refl. 
+
+Admitted.
+
+
+Lemma ge_lub_right:
+  forall x y, ge (lub x y) y.
+Proof. Admitted.
+End LPMap1.
+
+
+
+Module LPMap(L: SEMILATTICE_WITH_TOP) <: SEMILATTICE_WITH_TOP.
+
+Inductive t' : Type :=
+  | Bot: t'
+  | Top_except: PCTree.t L.t -> t'.
+
+Definition t: Type := t'.
+
+Definition get (p: pc) (x: t) : L.t :=
+  match x with
+  | Bot => L.bot
+  | Top_except m => match m!p with None => L.top | Some x => x end
+  end.
+
+Definition set (p: pc) (v: L.t) (x: t) : t :=
+  match x with
+  | Bot => Bot
+  | Top_except m =>
+      if L.beq v L.bot
+      then Bot
+      else Top_except (if L.beq v L.top then PCTree.remove p m else PCTree.set p v m)
+  end.
+
+Lemma gsspec:
+  forall p v x q,
+  x <> Bot -> ~L.eq v L.bot ->
+  L.eq (get q (set p v x)) (if PC.eqb q p then v else get q x).
+Proof.
+  intros. unfold set. destruct x. congruence.
+  destruct (L.beq v L.bot) eqn:EBOT.
+  elim H0. apply L.beq_correct; auto.
+  destruct (L.beq v L.top) eqn:ETOP; simpl.
+  rewrite PCTree.grspec. 
+
+destruct ( PCTree.elt_eq q p). subst. unfold PC.eqb. 
+destruct ( PC.eq_dec p p).
+apply L.eq_sym. eapply L.beq_correct. eauto. contradiction n; eauto.
+
+
+
+unfold PC.eqb. simpl in *. destruct ( PC.eq_dec q p). subst. contradiction n; eauto.
+apply L.eq_refl.
+
+
+
+
+
+
+  rewrite PCTree.gsspec. 
+destruct ( PCTree.elt_eq q p). subst. unfold PC.eqb. destruct (PC.eq_dec p p). eapply L.eq_refl. contradiction n; eauto. unfold PC.eqb. destruct (PC.eq_dec q p). subst. contradiction n; eauto. apply L.eq_refl. Qed.
+
+
+Definition eq (x y: t) : Prop :=
+  forall p, L.eq (get p x) (get p y).
+
+Lemma eq_refl: forall x, eq x x.
+Proof.
+  intros. unfold eq. simpl in *. intros. apply L.eq_refl. Qed.
+
+
+
+
+Lemma eq_sym: forall x y, eq x y -> eq y x.
+Proof.
+intros. unfold eq in *. intros. eapply L.eq_sym.   eauto. Qed.
+
+Lemma eq_trans: forall x y z, eq x y -> eq y z -> eq x z.
+Proof.
+unfold eq. intros. eapply L.eq_trans; eauto. Qed.
+
+Definition beq (x y: t) : bool :=
+  match x, y with
+  | Bot, Bot => true
+  | Top_except m, Top_except n => PCTree.beq L.beq m n
+  | _, _ => false
+  end.
+
+Lemma beq_correct: forall x y, beq x y = true -> eq x y.
+Proof.
+  destruct x; destruct y; simpl; intro; try congruence.
+  apply eq_refl.
+  red; intro; simpl.
+  rewrite PCTree.beq_correct in H. generalize (H p).
+  destruct (t0!p); destruct (t1!p); intuition.
+  apply L.beq_correct; auto.
+  apply L.eq_refl.
+Qed.
+  
+Definition ge (x y: t) : Prop :=
+  forall p, L.ge (get p x) (get p y).
+
+Lemma ge_refl: forall x y, eq x y -> ge x y.
+Proof.
+  unfold ge, eq; intros. apply L.ge_refl. auto.
+Qed.
+
+
+Lemma ge_trans: forall x y z, ge x y -> ge y z -> ge x z.
+Proof.
+  unfold ge; intros. apply L.ge_trans with (get p y); auto.
+Qed.
+
+
+Definition bot := Bot.
+
+Lemma get_bot: forall p, get p bot = L.bot.
+Proof.
+  unfold bot; intros; simpl. auto.
+Qed.
+
+Lemma ge_bot: forall x, ge x bot.
+Proof.
+  unfold ge; intros. rewrite get_bot. apply L.ge_bot.
+Qed.
+
+
+Definition top := Top_except (PCTree.empty L.t).
+
+Lemma get_top: forall p, get p top = L.top.
+Proof.
+  unfold top; intros; simpl. eauto. 
+Qed.
+
+
+Lemma ge_top: forall x, ge top x.
+Proof.
+  unfold ge; intros. rewrite get_top. apply L.ge_top.
+Qed.
+
+
+Module LM := LPMap1(L).
+
+Definition opt_lub (x y: L.t) : option L.t :=
+  let z := L.lub x y in
+  if L.beq z L.top then None else Some z.
+
+Definition lub (x y: t) : t :=
+  match x, y with
+  | Bot, _ => y
+  | _, Bot => x
+  | Top_except m, Top_except n =>
+      Top_except
+        (PCTree.combine
+           (fun a b =>
+              match a, b with
+              | Some u, Some v => opt_lub u v
+              | _, _ => None
+              end)
+           m n)
+  end.
+(*
+Lemma gcombine_top:
+  forall f t1 t2 p,
+  f None None = None ->
+  L.eq (get p (Top_except (PCTree.combine f t1 t2)))
+       (match f t1!p t2!p with Some x => x | None => L.top end).
+Proof.
+*)
+Lemma ge_lub_left:
+  forall x y, ge (lub x y) x.
+Proof. Admitted.
+
+Lemma ge_lub_right:
+  forall x y, ge (lub x y) y.
+Proof.
+Admitted.
+End LPMap.
+
+
+
+
+
+
+Module lidPMap(L: SEMILATTICE_WITH_TOP) <: SEMILATTICE_WITH_TOP.
+
+Inductive t' : Type :=
+  | Bot: t'
+  | Top_except: lidTree.t L.t -> t'.
+
+Definition t: Type := t'.
+
+Definition get (p: local_id) (x: t) : L.t :=
+  match x with
+  | Bot => L.bot
+  | Top_except m => match lidTree.get p m with None => L.top | Some x => x end
+  end.
+
+Definition set (p: local_id) (v: L.t) (x: t) : t :=
+  match x with
+  | Bot => Bot
+  | Top_except m =>
+      if L.beq v L.bot
+      then Bot
+      else Top_except (if L.beq v L.top then lidTree.remove p m else lidTree.set p v m)
+  end.
+Definition eq (x y: t) : Prop :=
+  forall p, L.eq (get p x) (get p y).
+
+Lemma gsspec:
+  forall p v x q,
+  x <> Bot -> ~L.eq v L.bot ->
+  L.eq (get q (set p v x)) (if loc_id_eq q p then v else get q x).
+Proof.
+  intros. unfold set. destruct x. congruence.
+  destruct (L.beq v L.bot) eqn:EBOT.
+  elim H0. apply L.beq_correct; auto.
+  destruct (L.beq v L.top) eqn:ETOP; simpl.
+  rewrite lidTree.grspec. unfold lidTree.elt_eq. destruct (loc_id_eq q p).
+  apply L.eq_sym. apply L.beq_correct; auto. eapply L.eq_refl. rewrite lidTree.gsspec.
+  unfold lidTree.elt_eq. destruct (loc_id_eq q p). eapply L.eq_refl. eapply L.eq_refl. Qed.
+
+
+
+
+
+  Lemma fgsspec:
+  forall p v x q,
+  x <> Bot -> ~L.eq v L.bot ->
+ L.eq (get q (set p v x)) (if loc_id_eq q p then v else get q x).
+Proof. intros.
+   unfold set. destruct x. congruence.
+  destruct (L.beq v L.bot) eqn:EBOT.
+  elim H0. apply L.beq_correct; auto.
+  destruct (L.beq v L.top) eqn:ETOP; simpl.
+  rewrite lidTree.grspec. unfold lidTree.elt_eq. destruct (loc_id_eq q p).
+  apply L.eq_sym. apply L.beq_correct; auto.
+  apply L.eq_refl.
+  rewrite lidTree.gsspec. destruct (lidTree.elt_eq q p). subst. destruct ( loc_id_eq p p). apply L.eq_refl. contradiction n; eauto. destruct (loc_id_eq q p). subst. contradiction n; eauto. apply L.eq_refl.
+Qed.
+
+
+  
+Lemma eq_refl: forall x, eq x x.
+Proof.
+unfold eq. intros. eapply L.eq_refl.
+Qed.
+
+Lemma eq_sym: forall x y, eq x y -> eq y x.
+Proof.
+unfold eq in *; intros. eapply L.eq_sym. eauto. Qed.
+
+
+
+  Lemma eq_trans: forall x y z, eq x y -> eq y z -> eq x z.
+Proof.
+unfold eq; intros. eapply L.eq_trans; eauto. Qed.
+
+
+  Definition beq (x y: t) : bool :=
+  match x, y with
+  | Bot, Bot => true
+  | Top_except m, Top_except n => lidTree.beq L.beq m n
+  | _, _ => false
+  end.
+
+Lemma beq_correct: forall x y, beq x y = true -> eq x y.
+Proof.
+  destruct x; destruct y; simpl; intro; try congruence.
+  apply eq_refl.
+  red; intro; simpl.
+  rewrite lidTree.beq_correct in H. generalize (H p).
+  destruct (t0 # p); destruct (t1 # p); intuition.
+  apply L.beq_correct; auto.
+  apply L.eq_refl.
+Qed.
+
+
+Definition ge (x y: t) : Prop :=
+  forall p, L.ge (get p x) (get p y).
+
+Lemma ge_refl: forall x y, eq x y -> ge x y.
+Proof.
+unfold eq, ge; intros. apply L.ge_refl. auto. Qed.
+
+Lemma ge_trans: forall x y z, ge x y -> ge y z -> ge x z.
+Proof.
+unfold ge. intros.  apply L.ge_trans with (get p y); auto.
+Qed.
+
+
+Definition bot := Bot.
+
+Lemma get_bot: forall p, get p bot = L.bot.
+Proof.
+  unfold bot; intros; simpl. auto.
+Qed.
+
+
+Lemma ge_bot: forall x, ge x bot.
+Proof.
+
+    unfold ge; intros. rewrite get_bot. apply L.ge_bot.
+Qed.
+
+
+
+Definition top := Top_except (lidTree.empty L.t).
+
+Lemma get_top: forall p, get p top = L.top.
+Proof.
+  unfold top; intros; simpl. eauto.
+   Qed.
+
+
+Lemma ge_top: forall x, ge top x.
+Proof. intros. unfold ge. intros. 
+ rewrite get_top. apply L.ge_top. Qed.
+
+
+Module LM := LPMap1(L).
+
+Definition opt_lub (x y: L.t) : option L.t :=
+  let z := L.lub x y in
+  if L.beq z L.top then None else Some z.
+
+Definition lub (x y: t) : t :=
+  match x, y with
+  | Bot, _ => y
+  | _, Bot => x
+  | Top_except m, Top_except n =>
+      Top_except
+        (lidTree.combine
+           (fun a b =>
+              match a, b with
+              | Some u, Some v => opt_lub u v
+              | _, _ => None
+              end)
+           m n)
+  end.
+(*
+Lemma gcombine_top:
+  forall f t1 t2 p,
+  f None None = None ->
+  L.eq (get p (Top_except (PCTree.combine f t1 t2)))
+       (match f t1!p t2!p with Some x => x | None => L.top end).
+Proof.
+*)
+Lemma ge_lub_left:
+  forall x y, ge (lub x y) x.
+Proof. Admitted.
+
+Lemma ge_lub_right:
+  forall x y, ge (lub x y) y.
+Proof.
+Admitted.
+End lidPMap.
