src/coq/optimisations/Kildall/static_eval_valueanalysis.v
@@ -1,0 +1,412 @@
+Require Import Vellvm.optimisations.Kildall.lattice.
+Require Import Vellvm.optimisations.maps.
+
+
+Require Import ZArith List String Omega.
+Require Import Vellvm.Ollvm_ast Vellvm.Classes Vellvm.Util Vellvm.CFGProp Vellvm.CFG.
+Require Import Vellvm.optimisations.transform.
+Require Import Vellvm.optimisations.paco_util.
+Require Import Vellvm.optimisations.step_trace.
+Require Import Vellvm.optimisations.EqNat.
+Require Import Vellvm.optimisations.Kildall.static_eval_valuedomain.
+Require Import Vellvm.optimisations.Kildall.kildall.
+
+Require Import Vellvm.DecidableEquality.
+Require Import Vellvm.DecidableProp.
+
+Require Import Coq.Logic.FunctionalExtensionality.
+Require Import paco.
+Require Import Vellvm.Memory.
+Require Import Vellvm.Effects.
+From mathcomp.ssreflect
+     Require Import ssreflect ssrbool seq eqtype ssrnat.
+
+
+
+Print NODE_SET.
+Module NodeSetForward <: NODE_SET.
+  Definition t := list pc.
+  Definition empty := nil : list pc.
+  Definition add (n: pc) (s: t) : t := n :: s.
+
+
+  
+  
+  Definition pick (s: t) :=
+    match s with
+    | nil => None
+    | hd :: tl => Some (hd, tl)
+    end.
+
+  
+  Definition code_to_pc (fn:function_id) (bk:block_id) (i:instr_id*instr) : pc := mk_pc fn bk (fst i).
+  Definition map_code fn bk (c:code) : seq pc := map (code_to_pc fn bk) c.
+  Definition block_to_pc fn (b:block) := map_code fn (blk_id b) (blk_code b) ++ (cons (mk_pc fn (blk_id b) (blk_term_id b)) nil).
+Print block_to_cmd. Print block.
+
+Lemma all_node_block : forall code fn n instr,  block_to_cmd code n = Some instr -> In (mk_pc fn (blk_id code) n) (block_to_pc fn code).
+Proof. intros. destruct code. simpl in *. unfold block_to_pc. simpl in *. unfold block_to_cmd in *. simpl in *. unfold blk_term_id in *. simpl in *. destruct blk_term. simpl in *.
+       destruct ( decide (i = n)). simpl in *. simpl in *. subst. induction blk_code. simpl in *. eauto. simpl in *. right. eauto. induction blk_code. simpl in *. inversion H. simpl in *. simpl in *. destruct a. simpl in *. destruct (decide (n = i0)). simpl in *. unfold code_to_pc. simpl in *. subst. left. eauto. right. eapply IHblk_code; eauto. Qed.
+
+
+
+
+
+Definition cfg_to_pc fn (c:cfg) := flatten (map (block_to_pc fn) (blks c)).
+Definition def_cfg_to_pc (d:definition cfg) := cfg_to_pc (dc_name (df_prototype d)) (df_instrs d).
+
+
+Print find_block.
+
+
+
+
+  Definition mcfg_to_pc (m:mcfg) := flatten (map def_cfg_to_pc (m_definitions m)).  
+
+
+Definition all_nodes (code: mcfg) := mcfg_to_pc code.
+  Definition In (p:pc) (l:t) := In p l.
+  Lemma empty_spec:
+    forall n, ~In n empty.
+Proof.
+intros. simpl in *. eauto. Qed.
+  Lemma add_spec:
+    forall n n' s, In n' (add n s) <-> n = n' \/ In n' s.
+Proof.
+  intros. simpl in *.  split; intros. eauto. eauto. Qed.
+
+  Lemma pick_none:
+    forall s n, pick s = None -> ~In n s.
+Proof.
+  intros. unfold not. intros. induction s. simpl in *. eauto. simpl in *. inversion H. Qed.
+
+  
+  Lemma pick_some:
+    forall s n s', pick s = Some(n, s') ->
+    forall n', In n' s <-> n = n' \/ In n' s'.  
+Proof.
+  intros until s'. induction s. simpl in *. intros. split. inversion H. inversion H. simpl in *. intros. inversion H. subst. split. intros. eauto. simpl in *. intros. eauto. Qed.
+
+Lemma all_nodes_spec:
+    forall code n instr,
+    fetch code n = Some instr -> In n (all_nodes code).
+Proof.
+  unfold fetch. unfold all_nodes. unfold mcfg_to_pc. simpl in *. unfold def_cfg_to_pc. simpl in *. unfold cfg_to_pc. simpl in *. unfold block_to_pc. simpl in *.
+simpl in *. destruct code. induction m_definitions. simpl in *. intros. destruct n. inversion H. 
+
+
+Admitted.
+
+
+
+
+End NodeSetForward.
+
+Module DS := Dataflow_Solver(VA)(NodeSetForward).
+
+
+Definition block_entry_pc (m:mcfg) (f:function_id) (b:block_id) :=
+  match find_block_entry m f b with
+  | Some (BlockEntry a p) => cons p nil
+                   | None => nil
+  end.
+
+
+Definition next_term (m:mcfg) (f:function_id) (t:terminator) :=
+  match t with
+  | TERM_Ret _ => nil
+  | TERM_Ret_void => nil
+  | TERM_Br _ br1 br2 => (block_entry_pc m f br1) ++ (block_entry_pc m f br2) 
+  | TERM_Br_1 br1 => (block_entry_pc m f br1) 
+  | _ => nil
+  end.
+
+
+
+Definition get_successors (m:mcfg) (p:pc) :=
+  match fetch m p with
+  | Some (Term a) => next_term m (fn p) a
+  | Some (CFG.Step (INSTR_Call (_, ID_Global fid) args)) => match incr_pc m p, find_function_entry m fid  with
+                         | None, None => nil
+                         | Some a, Some (FunctionEntry _ b) => cons a (cons b nil)
+                         | Some a, _ => cons a nil
+                         | None, Some (FunctionEntry _ a) => cons a nil
+                                                
+                         end
+  | Some (CFG.Step a) => match incr_pc m p with
+                         | None => nil
+                         | Some a => cons a nil
+                         end
+  | None => nil 
+  end.
+
+
+
+
+Print instr. Print Expr. Print aval.
+       
+
+Definition transfer' (m:mcfg) (p:pc) (a:aenv) : VA.t :=
+  match fetch m p with
+  | Some (Term (TERM_Br _ _ _)) => VA.State (AE.Top_except nil)
+  | Some (Term (TERM_Br_1 _)) => VA.State (AE.Top_except nil)
+  | Some (CFG.Step (INSTR_Op (SV (VALUE_Integer i)))) => match (pt p) with
+                                                         | IId id => VA.State (AE.set id (avalue (DV (VALUE_Integer i))) a)
+                                                         | _ => VA.State a
+                                                         end
+                                                           
+    
+  | Some (CFG.Step (INSTR_Call _ _)) => VA.State (AE.Top_except nil)
+  | Some _ => match (pt p) with
+              | IId id => VA.State (AE.set id (vtop) a)
+
+              | _ => VA.State a
+              end
+                
+  | None => VA.State a
+  end.
+
+Definition transfer (m:mcfg) (p:pc) (v:VA.t)  : VA.t :=
+  match v with
+  | VA.Bot => VA.Bot
+  | VA.State ae => match transfer' m p ae with
+                   | VA.Bot => VA.Bot
+                   | VA.State ae' => VA.State ae'
+                   end
+                     
+  end.
+
+
+Definition find_func (m:mcfg) :=
+  match find_function_entry m (Name "main") with
+   | Some (FunctionEntry _ p) => Some p
+   | None => None                
+  end.
+
+
+Definition analyse (m:mcfg) :=
+  match find_func m with
+  | Some start_pc => match (DS.fixpoint m fetch get_successors transfer start_pc (VA.State (AE.Bot))) with
+                     | Some res => res
+                     | None => PCMap.init (VA.State (AE.top))
+                     end
+                       
+  | None =>  PCMap.init (VA.State (AE.top))
+  end.
+
+
+
+Definition lookup_env_aenv (e:env) (id:raw_id) : aval :=
+  match lookup_env e id with
+  | None => vbot
+  | Some a => avalue a
+  end.
+
+
+
+(*env - aenv*)
+Inductive vmatch : aval -> aval -> Prop :=
+| vtop_match : forall dval, vmatch dval vtop
+| vval_match : forall dval dval1, dval = dval1 -> vmatch (avalue dval1) (avalue dval).
+
+
+
+
+Definition ematch (e:env) (a:aenv) := forall p, vmatch (lookup_env_aenv e p) (AE.get p a).
+
+Inductive vge: aval -> aval -> Prop :=
+| vge_bot : forall v, vge v vbot
+| vge_val : forall v v1, v = v1 -> vge (avalue v) (avalue v1)
+| vge_top : forall v, vge vtop v.
+
+
+
+
+
+Lemma vmatch_ge:
+  forall v x y, vge x y -> vmatch v y -> vmatch v x.
+Proof.
+  induction 1; intros V. inversion V. subst. eauto. constructor. Qed.
+
+
+
+Lemma ematch_ge:
+  forall  e ae1 ae2,
+  ematch e ae1 -> AE.ge ae2 ae1 -> ematch e ae2.
+Proof. intros. unfold ematch in *. intros. unfold AE.ge in *. specialize (H p).
+       specialize (H0 p). unfold AVal.ge in *. simpl in *. destruct ((lookup_env_aenv e p)); eauto. eapply vmatch_ge; eauto. destruct ( AE.get p ae2); simpl in *; eauto. destruct ( AE.get p ae1); eauto. apply vge_bot. inversion H0. inversion H0. destruct (AE.get p ae1). constructor. constructor. destruct (decide (n = n0)). subst; eauto. simpl in *. inversion H0. inversion H0.
+destruct (AE.get p ae1). constructor. constructor. constructor.
+destruct (AE.get p ae1), ( AE.get p ae2); eauto; inversion H; inversion H0; subst. constructor.
+destruct (decide (n1 = n)). subst. eauto. simpl in *. inversion H5. constructor. 
+destruct ( AE.get p ae2), (AE.get p ae1); try constructor; eauto; try inversion H0; inversion H. Qed.
+
+
+
+Lemma vmatch_false : forall e p, vmatch (lookup_env_aenv e p) AVal.bot -> False.
+Proof. intros. inversion H. Qed.
+
+
+Lemma ematch_update:
+  forall e ae v av r,
+  ematch e ae -> vmatch (avalue v) av -> ematch (add_env r v e) (AE.set r av ae).
+Proof.
+  intros. red. intros. remember ( (lookup_env_aenv (add_env r v e) p)).
+ assert  (ae <> AE.Bot -> ~ (AVal.beq av AVal.bot) = true ->
+vmatch a ((if loc_id_eq p r then av else AE.get p ae)) -> vmatch a (AE.get p (AE.set r av ae))).
+ intros. unfold is_left in. simpl in *. unfold AE.get, AE.set in *. unfold is_left in *. simpl in *. destruct ae. congruence. destruct ( AVal.beq av AVal.bot). contradiction H2; eauto.
+ destruct (AVal.beq av AVal.top) eqn:?. simpl in *.
+ rewrite lidTree.grspec. unfold lidTree.elt_eq. 
+destruct ( loc_id_eq p r). constructor. eauto.
+rewrite lidTree.gsspec. unfold lidTree.elt_eq. simpl in *.
+destruct ( loc_id_eq p r). eauto. eauto.
+apply H1. unfold not. intros. subst. unfold ematch in *.
+simpl in *. specialize (H r). inversion H. simpl in *.
+unfold not. intros.  apply AVal.beq_eq in H2.
+subst. simpl in *. inversion H0.
+unfold is_left. simpl in *. subst.
+unfold lookup_env_aenv, add_env, lookup_env in *; simpl in *.
+destruct (AstLib.RawID.eq_dec p r), (loc_id_eq p r); subst; eauto; try contradiction n; eauto.
+Qed.
+
+
+
+ 
+Inductive sound_stack : mcfg -> stack -> Prop :=
+| nil_stack : forall p, sound_stack p nil
+| kret_stack : forall id m p e k ae
+(AN: (analyse m)!!(mk_pc (fn p) (bk p) (IId id)) = VA.State ae)
+(EM: ematch e ae)  (stk:sound_stack m k),
+    (exists tptr tval, fetch m (mk_pc (fn p) (bk p) (IId id)) = Some (CFG.Step (INSTR_Call tptr tval)) /\incr_pc m (mk_pc (fn p) (bk p) (IId id)) = Some p) -> sound_stack m ((KRet e id p)::k)
+| kret_void_stack : forall m p e k ae (stk:sound_stack m k),
+    (exists tptr tval id, (analyse m)!!(mk_pc (fn p) (bk p) (IVoid id)) = VA.State ae /\ ematch e ae /\ fetch m (mk_pc (fn p) (bk p) (IVoid id)) = Some (CFG.Step (INSTR_Call tptr tval)) /\
+                          incr_pc m (mk_pc (fn p) (bk p) (IVoid id)) = Some p)  -> sound_stack m ((KRet_void e p)::k).
+
+
+Inductive sound_state : mcfg -> state -> Prop :=
+| sound_state_intro :
+    forall m st  ae
+           (sstack: sound_stack m (stack_of st))
+(AN: (analyse m)!!(pc_of st) = VA.State ae)
+(EM: ematch (env_of st) ae) ,
+      sound_state m st.
+
+
+
+
+Lemma analyse_successor:
+  forall m n ae ae' s instr,
+    (analyse m)!!n = VA.State ae ->
+    fetch m n = Some instr ->
+    In s (get_successors m n) ->
+    transfer' m n ae = ae' ->
+    VA.ge (analyse m)!!s (transfer m n (VA.State ae)).
+Proof. unfold analyse; intros. unfold find_func in *. simpl in *.
+       unfold find_function_entry in *. simpl in *.
+       destruct ( find_function m (Name "main")) eqn:?.
+       destruct ( find_block (blks (df_instrs d)) (init (df_instrs d))) eqn:?.
+       remember ( (VA.State AE.Bot)) as entry.
+       destruct ( DS.fixpoint m fetch get_successors transfer  {| fn := Name "main"; bk := init (df_instrs d); pt := blk_entry_id b |} entry) eqn:?.
+       assert (A: VA.ge t !! s (transfer m n (t !!n))).
+       eapply DS.fixpoint_solution; eauto with coqlib. intros.
+       unfold transfer. apply DS.L.eq_refl. rewrite H in A.
+       unfold transfer in A. unfold transfer in H2. rewrite H2 in A.
+       rewrite H2. unfold transfer.  eauto. simpl in *.
+       destruct (transfer' m n ae). eauto. apply AE.ge_top. rewrite H2.
+       simpl in *. destruct ae'.  eauto. eapply AE.ge_top. simpl in *.
+       rewrite H2. destruct ae'. simpl in *. eauto. eapply AE.ge_top. Qed.
+
+
+
+Lemma analyse_succ:
+  forall e f n ae instr s ae',
+  (analyse f)!!n = VA.State ae ->
+  fetch f n = Some instr ->
+  In s (get_successors f n) ->
+  transfer' f n ae = VA.State ae' ->
+  ematch e ae' ->
+  exists ae'',
+     (analyse f)!!s = VA.State ae''
+  /\ ematch e ae''.
+Proof. intros. generalize H; intros. eapply analyse_successor in H4; eauto.
+       unfold transfer in H4. simpl in *. rewrite H2 in H4.
+       destruct ((analyse f) !! s); try tauto. exists ae0.
+       split. auto. eapply ematch_ge; eauto. Qed. 
+
+
+Lemma sound_succ_state:
+  forall pc ae instr f s pc' e' ae',
+    (analyse f)!!pc = VA.State ae  ->
+    fetch f pc = Some instr -> In pc' (get_successors f pc) ->
+    transfer' f pc ae = VA.State ae' ->
+ematch e' ae' -> sound_stack f s ->
+  sound_state f (pc', e', s).
+Proof.
+  intros. generalize H. intros. eapply analyse_succ in H5; eauto.
+  generalize H5. intros (aea' & aef). destruct aef.
+  simpl in *. inversion H5. destruct H8. simpl in *. econstructor; eauto. Qed.
+
+
+Lemma unfold_fetch : forall m fn0 d bk0 b id  pt0 instr
+  (Heqo : find_function m fn0 = Some d)
+  (Heqo0 : find_block (blks (df_instrs d)) bk0 = Some b)
+  (Heqo1 : block_to_cmd b id = Some (instr, pt0)),
+  fetch m {| fn := fn0; bk := bk0; pt := id|} = Some instr.
+Proof. intros. unfold fetch. simpl in *. rewrite Heqo. rewrite Heqo0. rewrite Heqo1. eauto.
+Qed.
+
+
+Hint Resolve unfold_fetch.
+
+
+
+Lemma unfold_instr : forall m fn0 d b id instruction pt0 bk0 (Heqo : find_function m fn0 = Some d)
+ ( Heqo0 : find_block (blks (df_instrs d)) bk0 = Some b)
+  (Heqo1 : block_to_cmd b id = Some (CFG.Step instruction, Some pt0)),
+  In {| fn := fn0; bk := bk0; pt := pt0 |}
+    (get_successors m {| fn := fn0; bk := bk0; pt := id |}).
+Proof. intros. unfold get_successors. simpl in *. rewrite Heqo. rewrite Heqo0.
+       rewrite Heqo1. destruct instruction; simpl in *; eauto. destruct fn.
+       destruct i. simpl in *. destruct ( find_function_entry m id0) eqn:?.
+       destruct f. simpl in *. eauto. simpl in *. eauto. simpl in *.
+       eauto. Qed.
+Hint Resolve unfold_instr.
+
+Lemma ematch_add : forall id e ae v 
+(EM : ematch e ae),
+              ematch ((id, v) :: e) (AE.set id vtop ae).
+Proof. intros. eapply ematch_update; eauto; try constructor. Qed.
+Hint Resolve ematch_add.
+
+Lemma ematch_top : forall e0, ematch e0 (AE.Top_except [::]).
+Proof. intros. constructor. Qed. Hint Resolve ematch_top.
+
+
+Lemma transfer_add :
+forall m fn0 d bk0 b ae op pt0 id, 
+find_function m fn0 = Some d ->
+find_block (blks (df_instrs d)) bk0 = Some b ->
+block_to_cmd b (IVoid id) = Some (CFG.Step (INSTR_Op op), Some pt0) ->
+transfer' m {| fn := fn0; bk := bk0; pt := IVoid id |} ae = VA.State ae.
+Proof. intros. unfold transfer'.
+       simpl in *. rewrite H. rewrite H0.
+       rewrite H1. destruct op; simpl in *. destruct e; eauto. Qed.
+Hint Resolve transfer_add.
+
+
+
+
+
+Lemma block_implies_successor : forall m fn0 d0 bk0 b0 id x x0 pt0,
+find_function m fn0 = Some d0 -> find_block (blks (df_instrs d0)) bk0 = Some b0 -> 
+block_to_cmd b0 id =
+Some (CFG.Step (INSTR_Call x x0), Some pt0) -> In  (mk_pc fn0 bk0 pt0) (get_successors m (mk_pc fn0 bk0 id)).
+Proof. intros. unfold get_successors. simpl in *.
+       rewrite H. rewrite H0. rewrite H1. destruct x.
+       destruct i. simpl in *. unfold find_function_entry in *.
+       simpl in *. destruct (find_function m id0) eqn:?.
+       destruct ( find_block (blks (df_instrs d)) (init (df_instrs d))) eqn:?.
+       simpl in *. eauto. simpl in *. eauto. simpl in *. eauto.
+       simpl in *. eauto.  Qed.
+     Hint Resolve block_implies_successor.
+
+               
