src/coq/optimisations/Kildall/static_eval_valuedomain.v
@@ -1,0 +1,213 @@
+Print nat.
+
+Require Import Vellvm.optimisations.Kildall.lattice.
+Require Import Vellvm.optimisations.maps.
+
+
+Require Import ZArith List String Omega.
+Require Import Vellvm.Ollvm_ast Vellvm.Classes Vellvm.Util Vellvm.CFGProp Vellvm.CFG.
+Require Import Vellvm.optimisations.transform.
+Require Import Vellvm.optimisations.paco_util.
+Require Import Vellvm.optimisations.step_trace.
+Require Import Vellvm.optimisations.EqNat.
+
+Require Import Vellvm.DecidableEquality.
+Require Import Vellvm.DecidableProp.
+
+Require Import Coq.Logic.FunctionalExtensionality.
+Require Import paco.
+Require Import Vellvm.Memory.
+Require Import Vellvm.Effects.
+From mathcomp.ssreflect
+Require Import ssreflect ssrbool seq eqtype ssrnat.
+(*ABSTRACT VALUES*)
+Inductive aval : Type :=
+  | vbot (* bottom (empty set of values) *)
+  | avalue (n: dvalue) (* exactly Vint n *)
+  | vtop
+. 
+
+
+
+Print eqType.
+Locate eqType.
+Print SEMILATTICE_WITH_TOP.
+Module AVal <: SEMILATTICE_WITH_TOP.
+
+  Definition t := aval.
+  Definition eq_val (a b:aval) :=
+    match a, b with
+    | vbot, vbot => True
+    | avalue n, avalue n1 =>  (n = n1)
+    | vtop, vtop => True
+    | _, _ => False                          
+    end.
+
+  Definition eq := eq_val.
+  Lemma eq_refl: forall x, eq x x.
+    Proof. intros. destruct x; simpl in *; eauto. Qed.
+Lemma eq_sym: forall x y, eq x y -> eq y x.
+Proof. intros. unfold eq in *. destruct x, y; simpl in *; eauto. Qed.
+
+
+Lemma eq_trans: forall x y z, eq x y -> eq y z -> eq x z.
+  Proof. intros. destruct x, y, z; simpl in *; eauto. inversion H. subst; eauto.  inversion H. Qed.
+
+  Lemma eq_val_correct : forall a b, eq_val a b  <-> a = b.
+  Proof. intros. destruct a, b; simpl in *; split; intros; eauto; inversion H; eauto. Qed.
+    Definition beq (a b:aval) :=
+      match a, b with
+    | vtop, vtop => true
+    | vbot, vbot => true
+    | avalue n, avalue n1 =>  decide (n = n1)
+    | _, _ => false                          
+    end.
+
+    Lemma beq_correct: forall x y, beq x y = true -> eq x y.
+    Proof. intros. destruct x, y; simpl in *; eauto. destruct (decide (n = n0)); simpl in *; eauto. inversion H. Qed.
+
+    Lemma beq_eq : forall x y, beq x y = true <-> x = y.
+    Proof. destruct x, y; simpl in *; intros; split; intros; eauto; inversion H. unfold decide in *. destruct (eq_dvalue n n0). subst. eauto. simpl in *. inversion H. subst. unfold decide. destruct ( eq_dvalue n0 n0); simpl in *. eauto. contradiction n; eauto. Qed.
+
+
+    
+(*a is greater or equal to b*)
+    Definition ge (a b: aval) : Prop :=
+      match a, b with
+      | vbot, vbot => True
+      | vbot, avalue _ => False
+      | vbot, vtop => False
+      | avalue _, vtop => False
+      | avalue _, vbot => True
+      | avalue v1, avalue v2 => decide (v1 = v2)
+      | vtop, vbot => True
+      | vtop, vtop => True
+                        
+      | vtop, avalue _  => True               
+      end.
+
+
+    Lemma ge_refl: forall x y, eq x y -> ge x y.
+    Proof. intros. destruct x, y; simpl in *; eauto.
+           +subst. unfold decide. destruct ( eq_dvalue n0 n0); simpl in *; eauto. Qed.
+        
+    Lemma ge_trans: forall x y z, ge x y -> ge y z -> ge x z.
+    Proof. intros. destruct x, y, z; simpl in *; eauto. unfold decide in *. destruct (eq_dvalue n n0); simpl in *; subst; eauto. Qed.
+
+    Definition top := vtop.
+    Definition bot := vbot.
+
+    Lemma ge_bot: forall x, ge x bot.
+    Proof. intros. destruct x; simpl in *; eauto. Qed.
+    
+
+Print aval.
+    Definition lub (a b: aval) :=
+      match a, b with
+      | vbot, _ => b
+      | _, vbot => a
+      | avalue v1, avalue v2 => if (decide (v1 = v2)) then avalue v1 else vtop
+      | avalue _, vtop => vtop
+      | vtop, avalue _ => vtop
+      | vtop, vtop => vtop
+      end.
+    
+    Lemma ge_lub_left: forall x y, ge (lub x y) x.
+    Proof. destruct x, y; simpl in *; eauto.
+           +unfold decide. destruct (  eq_dvalue n n); simpl in *; eauto.
+           +unfold is_left. unfold decide. simpl in *. destruct ( eq_dvalue n n0); simpl in *; eauto. unfold decide. destruct ( eq_dvalue n n); simpl in *; eauto. Qed.
+
+
+
+    
+    Lemma ge_lub_right: forall x y, ge (lub x y) y.
+    Proof. destruct x, y; simpl in *; eauto.
+           unfold decide. destruct ( eq_dvalue n n); simpl in *; eauto. unfold is_left. 
+unfold decide. destruct (eq_dvalue n n0); simpl in *; subst; eauto. unfold decide.
+ destruct ( eq_dvalue n0 n0); simpl in *; eauto. Qed.
+
+
+ Lemma ge_top: forall x, ge top x.
+Proof. destruct x; simpl in *; eauto. Qed.
+       
+End AVal.
+
+Module AE := lidPMap(AVal).
+
+Definition aenv := AE.t.
+
+
+Module VA <: SEMILATTICE.
+
+  Inductive t' := Bot | State (ae: aenv).
+  Definition t := t'.
+
+  Definition eq (x y: t) :=
+    match x, y with
+    | Bot, Bot => True
+    | State ae1, State ae2 => AE.eq ae1 ae2
+    | _, _ => False
+    end.
+
+  Lemma eq_refl: forall x, eq x x.
+Proof.
+  intros.
+destruct x. simpl in *. eauto. simpl in *. apply AE.eq_refl. Qed.
+
+  Lemma eq_sym: forall x y, eq x y -> eq y x.
+  Proof. intros.  destruct x, y; simpl in *; eauto. apply AE.eq_sym in H. auto. Qed.
+
+  Lemma eq_trans: forall x y z, eq x y -> eq y z -> eq x z.
+Proof.
+Admitted.
+
+
+Definition beq (x y: t) : bool :=
+    match x, y with
+    | Bot, Bot => true
+    | State ae1, State ae2 => AE.beq ae1 ae2
+    | _, _ => false
+    end.
+
+  Lemma beq_correct: forall x y, beq x y = true -> eq x y.
+Proof. Admitted.
+
+  Definition ge (x y: t) : Prop :=
+    match x, y with
+    | _, Bot => True
+    | Bot, _ => False
+    | State ae1, State ae2 => AE.ge ae1 ae2
+    end.
+
+  Lemma ge_refl: forall x y, eq x y -> ge x y.
+Proof.
+Admitted.
+
+Lemma ge_trans: forall x y z, ge x y -> ge y z -> ge x z.
+Proof.
+Admitted.
+
+
+  Definition bot : t := Bot.
+  Lemma ge_bot: forall x, ge x bot.
+Proof.
+Admitted.
+
+
+Definition lub (x y: t) : t :=
+    match x, y with
+    | Bot, _ => y
+    | _, Bot => x
+    | State ae1, State ae2 => State (AE.lub ae1 ae2)
+    end.
+
+  Lemma ge_lub_left: forall x y, ge (lub x y) x.
+Proof.
+Admitted.
+
+
+Lemma ge_lub_right: forall x y, ge (lub x y) y.
+Proof.
+Admitted.
+
+End VA.
