src/coq/optimisations/vellvm_tactics.v
@@ -1,0 +1,4 @@
+Ltac dupl x := generalize x; intro.
+Ltac contra_destr x := remember x; destruct x; try contradiction; auto.
+Ltac save_destr x := remember x; destruct x.
+Ltac inv x := inversion x; subst; auto.
